ECCA_core.v
@@ -1,0 +1,434 @@
+Require Export Atom.
+
+(* 
+=====================================
+=======--ECCA Definition--=========== 
+=====================================
+*)
+
+Declare Scope ECCA_scope.
+Delimit Scope ECCA_scope with ECCA.
+
+(* Restricted ECCA, used in computing *)
+
+Inductive ECCAval: Type :=
+  | Id (x: atom)
+  | Uni (U: ECCuni)
+  | Pi (x: atom) (A B: ECCAconf)
+  | Abs (x: atom) (A B: ECCAconf)
+  | Sig (x: atom) (A B: ECCAconf)
+  | Pair (v1 v2: ECCAval) (A: ECCAconf)
+  | Tru
+  | Fls
+  | Bool
+with
+ECCAconf: Type :=
+  | Comp (e: ECCAcomp)
+  | Let (x: atom) (A: ECCAcomp) (B: ECCAconf)
+(*   | If (v: ECCAval) (m1 m2: ECCAconf) *)
+with
+ECCAcomp: Type :=
+  | App (v1 v2: ECCAval)
+  | Val (v: ECCAval)
+  | Fst (v: ECCAval)
+  | Snd (v: ECCAval)
+(*   | Subst (x arg body: ECCAval) *)
+.
+
+Hint Constructors ECCAval. 
+Coercion Id: atom >-> ECCAval.
+Bind Scope ECCA_scope with ECCAval.
+Bind Scope ECCA_scope with ECCAconf.
+Bind Scope ECCA_scope with ECCAcomp.
+
+
+Inductive ECCAexp: Type :=
+  | eId (x: atom)
+  | eUni (U: ECCuni)
+  | ePi (x: atom) (A B: ECCAexp)
+  | eAbs (x: atom) (A B: ECCAexp)
+  | eSig (x: atom) (A B: ECCAexp)
+  | ePair (v1 v2: ECCAexp) (A: ECCAexp)
+  | eTru
+  | eFls
+  | eBool
+  | eLet (x: atom) (A: ECCAexp) (B: ECCAexp)
+(*   | eIf (v: ECCAexp) (m1 m2: ECCAexp) *)
+  | eApp (v1 v2: ECCAexp)
+  | eFst (v: ECCAexp)
+  | eSnd (v: ECCAexp)
+(*   | eSubst (x arg body: ECCAexp) *)
+.
+
+Hint Constructors ECCAexp.
+
+Inductive ECCAenv: Type :=
+  | Empty
+  | Assum (g: ECCAenv) (x: atom) (A: ECCAexp)
+  | Def (g: ECCAenv) (x: atom) (v: ECCAexp)
+  | Eq (g: ECCAenv) (v1 v2: ECCAexp)
+.
+Hint Constructors ECCAenv. 
+Notation "g ',' x '=' e" := (Def g x e) (at level 50, x at level 50): ECCA_scope.
+Notation "g ',' x ':' e" := (Assum g x e) (at level 50, x at level 50): ECCA_scope.
+
+(* 
+============================================================
+=======--Moving from restricted to unrestricted--=========== 
+============================================================
+*)
+
+Fixpoint flattenECCAval (e: ECCAval): ECCAexp :=
+match e with
+  | Id x => eId x
+  | Uni U => eUni U
+  | Pi x A B => ePi x (flattenECCAconf A) (flattenECCAconf B) 
+  | Abs x A B => eAbs x (flattenECCAconf A) (flattenECCAconf B)
+  | Sig x A B => eSig x (flattenECCAconf A) (flattenECCAconf B)
+  | Pair v1 v2 A => ePair (flattenECCAval v1) (flattenECCAval v2) (flattenECCAconf A)
+  | Tru => eTru
+  | Fls => eFls
+  | Bool => eBool
+end
+with flattenECCAcomp (e: ECCAcomp): ECCAexp :=
+match e with
+  | App v1 v2 => eApp (flattenECCAval v1) (flattenECCAval v2)
+  | Val v => flattenECCAval v
+  | Fst v => eFst (flattenECCAval v)
+  | Snd v => eSnd (flattenECCAval v)
+(*   | Subst x arg body => eSubst (flattenECCAval x) (flattenECCAval arg) (flattenECCAval body) *)
+end
+with flattenECCAconf (e: ECCAconf): ECCAexp :=
+match e with
+  | Comp e => flattenECCAcomp e
+  | Let x A B => eLet x (flattenECCAcomp A) (flattenECCAconf B)
+(*   | If v m1 m2 => eIf (flattenECCAval v) (flattenECCAconf m1) (flattenECCAconf m2) *)
+end.
+
+Fixpoint getECCAval (e: ECCAexp): option ECCAval :=
+match e with
+  | eId x => Some (Id x)
+  | eUni U => Some (Uni U)
+  | ePi x A B => 
+      let A := (getECCAconf A) in
+      let B := (getECCAconf B) in
+      match A with
+        | Some A => match B with
+          | Some B => Some (Pi x A B)
+          | None => None
+          end
+        | None => None
+        end
+  | eAbs x A B =>
+      let A := (getECCAconf A) in
+      let B := (getECCAconf B) in
+      match A with
+        | Some A => match B with
+          | Some B => Some (Abs x A B)
+          | None => None
+          end
+        | None => None
+        end
+  | eSig x A B =>
+      let A := (getECCAconf A) in
+      let B := (getECCAconf B) in
+      match A with
+        | Some A => match B with
+          | Some B => Some (Sig x A B)
+          | None => None
+          end
+        | None => None
+        end
+  | ePair v1 v2 A => 
+      let v1 := (getECCAval v1) in
+      let v2 := (getECCAval v2) in
+      let A  := (getECCAconf A) in
+      match v1 with
+        | Some v1 => match v2 with
+          | Some v2 => match A with 
+            | Some A => Some (Pair v1 v2 A)
+            | None => None
+            end
+          | None => None
+          end
+        | None => None
+        end
+  | eTru => (Some Tru)
+  | eFls => (Some Fls)
+  | eBool => (Some Bool)
+  | _ => None
+end
+with getECCAconf (e: ECCAexp): option ECCAconf :=
+match e with
+  | eLet x A B => 
+      let A := (getECCAcomp A) in
+      let B := (getECCAconf B) in
+      match A with
+        | Some A => match B with
+          | Some B => Some (Let x A B)
+          | None => None
+          end
+        | None => None
+        end
+(*   | eIf v m1 m2 =>
+      let m1 := (getECCAconf m1) in
+      let m2 := (getECCAconf m2) in
+      let v  := (getECCAval v) in
+      match m1 with
+        | Some m1 => match m2 with
+          | Some m2 => match v with 
+            | Some v => Some (If v m1 m2)
+            | None => None
+            end
+          | None => None
+          end
+        | None => None
+        end *)
+(* Computations are also configurations *)
+  | eApp v1 v2 =>
+      let v1 := (getECCAval v1) in
+      let v2 := (getECCAval v2) in
+      match v1 with
+        | Some v1 => match v2 with
+          | Some v2 => Some (Comp (App v1 v2))
+          | None => None
+          end
+        | None => None
+        end
+  | eFst v =>
+      let v := (getECCAval v) in
+      match v with
+        | Some v => Some (Comp (Fst v))
+        | None => None
+        end
+  | eSnd v =>
+      let v := (getECCAval v) in
+      match v with
+        | Some v => Some (Comp (Snd v))
+        | None => None
+        end
+(*   | eSubst x arg body =>
+      let x := (getECCAval x) in
+      let arg := (getECCAval arg) in
+      let body  := (getECCAval body) in
+      match x with
+        | Some x => match arg with
+          | Some arg => match body with 
+            | Some body => Some (Comp (Subst x arg body))
+            | None => None
+            end
+          | None => None
+          end
+        | None => None
+        end   *)
+(* Values are also computations which are also configurations *)
+  | eId x => Some (Comp (Val (Id x)))
+  | eUni U => Some (Comp (Val (Uni U)))
+  | ePi x A B => 
+      let A := (getECCAconf A) in
+      let B := (getECCAconf B) in
+      match A with
+        | Some A => match B with
+          | Some B => Some (Comp (Val (Pi x A B)))
+          | None => None
+          end
+        | None => None
+        end
+  | eAbs x A B =>
+      let A := (getECCAconf A) in
+      let B := (getECCAconf B) in
+      match A with
+        | Some A => match B with
+          | Some B => Some (Comp (Val (Abs x A B)))
+          | None => None
+          end
+        | None => None
+        end
+  | eSig x A B =>
+      let A := (getECCAconf A) in
+      let B := (getECCAconf B) in
+      match A with
+        | Some A => match B with
+          | Some B => Some (Comp (Val (Sig x A B)))
+          | None => None
+          end
+        | None => None
+        end
+  | ePair v1 v2 A => 
+      let v1 := (getECCAval v1) in
+      let v2 := (getECCAval v2) in
+      let A  := (getECCAconf A) in
+      match v1 with
+        | Some v1 => match v2 with
+          | Some v2 => match A with 
+            | Some A => Some (Comp (Val (Pair v1 v2 A)))
+            | None => None
+            end
+          | None => None
+          end
+        | None => None
+        end
+  | eTru => (Some (Comp (Val Tru)))
+  | eFls => (Some (Comp (Val Fls)))
+  | eBool => (Some (Comp (Val Bool)))
+end
+with getECCAcomp (e: ECCAexp): option ECCAcomp :=
+match e with
+  | eApp v1 v2 =>
+      let v1 := (getECCAval v1) in
+      let v2 := (getECCAval v2) in
+      match v1 with
+        | Some v1 => match v2 with
+          | Some v2 => Some (App v1 v2)
+          | None => None
+          end
+        | None => None
+        end
+  | eFst v =>
+      let v := (getECCAval v) in
+      match v with
+        | Some v => Some (Fst v)
+        | None => None
+        end
+  | eSnd v =>
+      let v := (getECCAval v) in
+      match v with
+        | Some v => Some (Snd v)
+        | None => None
+        end
+(*   | eSubst x arg body =>
+      let x := (getECCAval x) in
+      let arg := (getECCAval arg) in
+      let body  := (getECCAval body) in
+      match x with
+        | Some x => match arg with
+          | Some arg => match body with 
+            | Some body => Some (Subst x arg body)
+            | None => None
+            end
+          | None => None
+          end
+        | None => None
+        end   *)
+(* Values are also computations *)
+  | eId x => Some (Val (Id x))
+  | eUni U => Some (Val (Uni U))
+  | ePi x A B => 
+      let A := (getECCAconf A) in
+      let B := (getECCAconf B) in
+      match A with
+        | Some A => match B with
+          | Some B => Some (Val (Pi x A B))
+          | None => None
+          end
+        | None => None
+        end
+  | eAbs x A B =>
+      let A := (getECCAconf A) in
+      let B := (getECCAconf B) in
+      match A with
+        | Some A => match B with
+          | Some B => Some (Val (Abs x A B))
+          | None => None
+          end
+        | None => None
+        end
+  | eSig x A B =>
+      let A := (getECCAconf A) in
+      let B := (getECCAconf B) in
+      match A with
+        | Some A => match B with
+          | Some B => Some (Val (Sig x A B))
+          | None => None
+          end
+        | None => None
+        end
+  | ePair v1 v2 A => 
+      let v1 := (getECCAval v1) in
+      let v2 := (getECCAval v2) in
+      let A  := (getECCAconf A) in
+      match v1 with
+        | Some v1 => match v2 with
+          | Some v2 => match A with 
+            | Some A => Some (Val (Pair v1 v2 A))
+            | None => None
+            end
+          | None => None
+          end
+        | None => None
+        end
+  | eTru => (Some (Val Tru))
+  | eFls => (Some (Val Fls))
+  | eBool => (Some (Val Bool))
+  | _ => None
+end
+.
+
+Definition isANF (e: ECCAexp): Prop :=
+  exists a, (getECCAconf e) = Some a.
+Definition isComp ( e: ECCAexp): Prop :=
+  exists a, (getECCAcomp e) = Some a.
+Definition isVal ( e: ECCAexp): Prop :=
+  exists a, (getECCAval e) = Some a.
+
+Coercion Val: ECCAval >-> ECCAcomp. 
+Coercion Comp: ECCAcomp >-> ECCAconf. 
+
+(* 
+=====================================
+=======--Type Environments --========
+=====================================
+*)
+
+Inductive ECCA_LookupTypeR : ECCAenv -> atom -> ECCAexp -> Prop:=
+  | aLT_gFirst (g': ECCAenv) (x: atom) (A: ECCAexp):
+      ECCA_LookupTypeR (Assum g' x A) x A
+  | aLT_AssumRest (g: ECCAenv) (x x': atom) (A a': ECCAexp):
+      ECCA_LookupTypeR g x A ->
+      (x <> x') ->
+      (ECCA_LookupTypeR (Assum g x' a') x A)
+  | aLT_DefRest (g: ECCAenv) (x x': atom) (A a': ECCAexp):
+      ECCA_LookupTypeR g x A ->
+  (*     (x <> x') -> *)
+      (ECCA_LookupTypeR (Def g x' a') x A)
+  | aLT_EqRest (g: ECCAenv) (x: atom) (v A v': ECCAexp):
+      ECCA_LookupTypeR g x A ->
+      ECCA_LookupTypeR (Eq g v v') x A 
+.
+Hint Constructors ECCA_LookupTypeR.
+
+
+Inductive ECCA_LookupDefR : ECCAenv -> atom -> ECCAexp -> Prop:=
+  | aLD_gFirst (g': ECCAenv) (x: atom) (e: ECCAexp) (A: ECCAexp):
+      ECCA_LookupDefR (Assum (Def g' x e) x A) x e
+  | aLD_AssumRest (g: ECCAenv) (x x': atom) (e: ECCAexp) (a': ECCAexp):
+      ECCA_LookupDefR g x e ->
+      (x <> x') ->
+      (ECCA_LookupDefR (Assum g x' a') x e)
+  | aLD_DefRest (g: ECCAenv) (x x': atom) (e e': ECCAexp):
+      ECCA_LookupDefR g x e ->
+      (x <> x') ->
+      (ECCA_LookupDefR (Def g x' e') x e)
+  | aLD_EqRest (g: ECCAenv) (x: atom) (v v': ECCAexp) (e: ECCAexp):
+      ECCA_LookupDefR g x e ->
+      ECCA_LookupDefR (Eq g v v') x e 
+.
+Hint Constructors ECCA_LookupDefR.
+
+
+(*should change val to conf *)
+Inductive ECCA_LookupEqR : ECCAenv -> ECCAexp -> ECCAexp -> Prop:=
+  | aLE_gFirst (g': ECCAenv) (v v': ECCAexp):
+    ECCA_LookupEqR (Eq g' v v') v v'
+  | aLE_AssumRest (g: ECCAenv) (x : atom) (v v' a: ECCAexp):
+      ECCA_LookupEqR g v v' ->
+      (ECCA_LookupEqR (Assum g x a) v v')
+  | aLE_DefRest (g: ECCAenv) (x: atom) (v v' e: ECCAexp):
+      ECCA_LookupEqR g v v' ->
+      (ECCA_LookupEqR (Def g x e) v v')
+  | aLE_EqRest (g: ECCAenv) (x: atom) (v1 v2 v1' v2': ECCAexp):
+      ECCA_LookupEqR g v1 v2 ->
+      (v1 <> v1') ->
+      ECCA_LookupEqR (Eq g v1' v2') v1 v2 
+.
+Hint Constructors ECCA_LookupEqR.
