ECCA_equiv_lemmas.v
@@ -1,0 +1,229 @@
+Require Export ECCA_equiv.
+Require Import ECCA_subst_lemmas.
+
+Lemma equiv_refl (g: ECCAenv) (A: ECCAexp):
+(g |- A =e= A)%ECCA.
+Proof.
+apply aE_Equiv with (e:= A); auto.
+Qed.
+
+(* 
+Lemma equiv_trans (g: ECCAenv) (A B C: ECCAexp):
+(g |- A =e= B ->
+g |- B =e= C ->
+g |- A =e= C)%ECCA.
+Proof.
+intros. inversion H; inversion H0; subst.
+- case (e = e0). *)
+
+Lemma aeq_fv_the_tough_part (x y : atom) (t1 t2 b1 b2 : ECCAexp)
+(H : x `notin` FV b2)
+(H0 : (b1 =a= swap y x b2)%ECCA)
+(H1 : (t1 =a= t2)%ECCA)
+(IHECCA_Aeq1 : FV b1 [=] FV (swap y x b2))
+(IHECCA_Aeq2 : FV t1 [=] FV t2):
+    union (FV t1) (remove x (FV b1)) 
+[=] union (FV t2) (remove y (FV b2)).
+Proof.
+unfold AtomSetImpl.Equal.
+    intro a.
+    repeat rewrite union_iff; repeat rewrite remove_iff.
+    rewrite IHECCA_Aeq1.
+    rewrite IHECCA_Aeq2.
+    split.
+    + intros [K1 | K2] .
+      * auto.
+      * destruct K2. apply (in_fv_equivariance y x) in H2.
+        rewrite swap_involutive in H2.
+        unfold swap_var in H2.
+        destruct (a == y); subst.
+          -- contradiction.
+          -- destruct (a == x); subst. 
+            ++ contradiction.
+            ++ right; split; auto.
+    + intros [K1 | K2].
+      * apply (in_fv_equivariance y x) in K1. 
+        pose (J := notin_fv_equivariance x y x b2 H). clearbody J.
+        unfold swap_var in *. destruct (a == y); subst.
+        -- destruct (x == y); subst.
+          ++ left. rewrite swap_id in K1. auto.
+          ++ destruct (x == x); try contradiction. left.
+              apply in_fv_equivariance with (x:= x) (y := y) in K1. 
+              rewrite swap_symmetric in K1. rewrite swap_involutive in K1.
+              unfold swap_var in K1. destruct (x == x) in K1; try contradiction.
+              apply K1.
+        -- destruct (a == x); destruct (x ==y); subst.
+          ++ rewrite swap_id in K1. left. apply K1.
+          ++ default_simp. left.
+             apply in_fv_equivariance with (x:= x) (y := y) in K1.
+             rewrite swap_symmetric in K1. rewrite swap_involutive in K1.
+             unfold swap_var in K1. default_simp. 
+          ++ rewrite swap_id in K1. left. apply K1.
+          ++ destruct (x==x) in J; try contradiction. apply notin_fv_equivariance with (x:= x) (y := y) in J.
+             rewrite swap_symmetric in J. rewrite swap_involutive in J.
+             unfold swap_var in J. default_simp.
+             apply in_fv_equivariance with (y:=x) (x:=y) in K1. 
+             rewrite swap_involutive in K1. unfold swap_var in K1. default_simp.
+      * right. destruct K2. split.
+        -- apply in_fv_equivariance with (x:=y) (y:=x) in H2. unfold swap_var in H2.
+           default_simp. apply in_fv_equivariance with (x:=y) (y:=x) in H2. 
+           rewrite swap_involutive in H2. unfold swap_var in H2. default_simp.
+        -- destruct (x==a). subst. contradiction. assumption.
+Qed.
+
+Lemma aeq_fv : forall t1 t2,
+    (t1 =a= t2 ->
+    FV t1 [=] FV t2)%ECCA.
+Proof.
+  induction 1; simpl in *; try fsetdec.
+  all: apply aeq_fv_the_tough_part; assumption.
+Qed.
+
+Lemma aeq_equivariance : forall x y t1 t2,
+    ECCA_Aeq t1 t2 ->
+    ECCA_Aeq (swap x y t1) (swap x y t2).
+Proof.
+  induction 1; intros; simpl in *; auto.
+  all: destruct (swap_var x y x0 == swap_var x y y0).
+  1,3,5,7: rewrite e; eapply aeq_abs_same || eapply aeq_pi_same 
+                   || eapply aeq_let_same || eapply aeq_sig_same;
+   auto; rewrite swap_equivariance in IHECCA_Aeq1; 
+   rewrite e in IHECCA_Aeq1; rewrite swap_id in IHECCA_Aeq1; auto.
+  all: rewrite swap_equivariance in IHECCA_Aeq1; 
+        eapply aeq_abs_diff || eapply aeq_pi_diff 
+     || eapply aeq_let_diff || eapply aeq_sig_diff;
+        try eapply notin_fv_nom_equivariance; auto.
+Qed.
+
+ Lemma aeq_sym_the_hard_part1
+(x y : atom)
+(t1 t2 b1 b2 : ECCAexp)
+(H : x `notin` FV b2)
+(H0 : (b1 =a= swap y x b2)%ECCA)
+(IHECCA_Aeq1 : (swap y x b2 =a= b1)%ECCA):
+y `notin` FV b1.
+Proof.
+apply notin_fv_equivariance_easy with (y:=y) in H. 
+  rewrite aeq_fv with (t1 := b1) (t2 := swap y x b2); auto. auto.
+Qed.
+
+ Lemma aeq_sym_the_hard_part2
+(x y : atom)
+(t1 t2 b1 b2 : ECCAexp)
+(H : x `notin` FV b2)
+(H0 : (b1 =a= swap y x b2)%ECCA)
+(IHECCA_Aeq1 : (swap y x b2 =a= b1)%ECCA):
+(b2 =a= swap x y b1)%ECCA.
+Proof.
+eapply aeq_equivariance with (x:=x) (y:=y) in IHECCA_Aeq1.
+  rewrite swap_symmetric in IHECCA_Aeq1.
+  rewrite swap_involutive with (x:=y) (y:=x) in IHECCA_Aeq1. auto.
+Qed.
+
+Lemma aeq_sym (A B: ECCAexp):
+(A =a= B ->
+B =a= A)%ECCA.
+Proof.
+intros. induction H.
+all: try auto.
+all: apply aeq_abs_diff || apply aeq_pi_diff || apply aeq_let_diff || apply aeq_sig_diff ; auto.
+all: apply aeq_sym_the_hard_part1 with (x:=x) (b2:=b2)
+  || apply aeq_sym_the_hard_part2 with (x:=x) (b2:=b2); auto.
+Qed.
+
+Lemma equiv_sym (g: ECCAenv) (A B: ECCAexp):
+(g |- A =e= B ->
+g |- B =e= A)%ECCA.
+Proof.
+intros. inversion H.
+- apply aE_Equiv with (e := e); auto.
+- subst. eapply aE_EquivIta2.
+  + auto.
+  + apply H1.
+  + apply H0.
+  + apply H2.
+- subst. eapply aE_EquivIta1.
+  + auto.
+  + apply H1.
+  + apply H0.
+  + apply H2.
+- apply aE_EquivAlpha; apply aeq_sym; auto.
+Qed.
+
+(* 
+Lemma equiv_distributes_over_pi (g: ECCAenv) (x: atom) (B B' A A': ECCAexp):
+(g |- A =e= A' ->
+g |- B =e= B' ->
+g |- ePi x A B =e= ePi x A' B')%ECCA.
+Proof.
+intros. inversion H. inversion H0.
+- subst.
+
+Lemma equiv_equivariant_over_subst (g: ECCAenv) (x: atom) (N N' A B: ECCAexp):
+(g |- N : A ->
+g |- N' : A ->
+g |- N =e= N' ->
+g |- (subst x N B) =e= (subst x N' B)
+)%ECCA.
+Proof.
+intros. induction H1. 
+- rewrite substWork_equation. rewrite substWork_equation.
+ destruct AtomSetImpl.mem.
+  + induction B; auto. destruct (x == x0); auto.
+    * eapply aE_Equiv with (e := e); auto.
+    * destruct (x == x0).
+      ++
+
+
+
+
+  + destruct (x == x0).
+    * apply H1.
+    * auto.
+  + destruct (x == x0).
+    * auto. Reset IHB2. inversion IHB1. 
+        --
+
+   
+- *)
+
+Lemma ECCA_Aeq_equivariance : forall x y t1 t2,
+    ECCA_Aeq t1 t2 ->
+    ECCA_Aeq (swap x y t1) (swap x y t2).
+Proof.
+  induction 1; intros; simpl in *; auto.
+  all: destruct (swap_var x y x0 == swap_var x y y0).
+  1,3,5,7: rewrite e; eapply aeq_abs_same || eapply aeq_pi_same || eapply aeq_let_same || eapply aeq_sig_same;
+   auto; 
+   rewrite swap_equivariance in IHECCA_Aeq1; rewrite e in IHECCA_Aeq1; rewrite swap_id in IHECCA_Aeq1; auto.
+  all: rewrite swap_equivariance in IHECCA_Aeq1; eapply aeq_abs_diff || eapply aeq_pi_diff || eapply aeq_let_diff || eapply aeq_sig_diff;
+      try eapply notin_fv_nom_equivariance; auto.
+Qed.
+
+Lemma capture_avoid_is_aeq_abs (xnew x: atom) (fvarg: atoms) (A e: ECCAexp):
+((let (xnew,_) := atom_fresh (union (fvarg) (FV e)) in
+                    (eAbs xnew A (swap x xnew e)))
+  =a=
+eAbs x A e)%ECCA.
+Proof.  destruct atom_fresh. intros. apply aeq_abs_diff.
+- fsetdec.
+- auto.
+- auto.
+Qed.
+
+(* Lemma subst_over_swap (x y z: atom) (A B: ECCAexp):
+(y <> x ->
+z `notin` FV B ->
+(subst y A B =a= B) ->
+(subst y A (swap x z B) =a= swap x z B))%ECCA.
+Proof.
+intros. inversion H1. 
+- subst. auto. rewrite H3.
+Admitted. *)
+
+Lemma subst_no_fv_aeq (y: atom) (A B: ECCAexp):
+(y `notin` (FV B) ->
+subst y A B =a= B)%ECCA.
+Proof.
+intros. rewrite not_mem_iff in H. rewrite substWork_equation. rewrite H. auto.
+Qed.
