ECCA_key_lemmas.v
@@ -1,0 +1,87 @@
+Require Export ECCA_typing.
+Require Export ECCA_equiv_lemmas.
+Require Export ECCA_subst_lemmas.
+
+Lemma Cut (g: ECCAenv) (K : ECCAcont) (N: ECCAexp) (A B B': ECCAexp):
+(ECCA_cont_has_type g K (Cont N A B) ->
+ECCA_has_type g N A ->
+exists B', ECCA_has_type g (fill_hole N K) B' /\ (B' =a= B))%ECCA.
+Proof. 
+intros. inversion H ; subst ; cbv.
+- exists B. split.
+  + eauto.
+  + eauto.
+- exists (subst y N B). split.
+  + eapply aT_Let with (n:= N) (m:= M) (A:=A) (B:=B) (x:=y) (g:=g).
+    * assumption.
+    * assumption.
+  + apply subst_no_fv_aeq. auto.
+Qed.
+
+Lemma equivalence_is_equivalence (g: ECCAenv) (y: atom) (N N' M: ECCAexp) (A B: ECCAexp):
+(g |- N : A ->
+g |- N' : A ->
+ECCA_Equiv g N N' ->
+
+((g, y = N), y : A) |- M : B ->
+((g, y = N'), y : A) |- M : B)%ECCA.
+Proof. (* intros. induction H2; default_simp.
+1: {shelve. } (* need to show that lookuptype is at most one to one *)
+6: {eapply aT_Let. 
+    - apply IHECCA_has_type1. 
+    - } *)
+Abort.
+
+Lemma Cut_modulo_equivalence (g: ECCAenv) (K : ECCAcont) (N N': ECCAexp) (A B B': ECCAexp):
+(ECCA_cont_has_type g K (Cont N A B) ->
+ECCA_has_type g N A ->
+ECCA_has_type g N' A ->
+ECCA_Equiv g N N' ->
+exists B', ECCA_has_type g (fill_hole N' K) B' /\ (B' =a= B))%ECCA.
+Proof. 
+intros. inversion H ; subst ; cbv.
+- exists B. split.
+  + eauto.
+  + eauto.
+- exists (subst y N' B). split.
+  + eapply aT_Let with (n:= N') (m:= M) (A:=A) (B:=B) (x:=y) (g:=g).
+    * assumption.
+    * shelve. (*  inversion H9 ; auto. 
+      -- subst. *)
+  + Abort. (* apply subst_no_fv_aeq. auto. *)
+
+
+
+(* | aT_Conv (g: ECCAenv) (e A B U: ECCAexp) :
+  (g |- e : A) ->
+  (g |- B : U) ->
+  (ECCA_sub_type g A B) ->
+  (g |- e : B)
+       
+Unable to unify "(g |- eLet y N M : subst y N B)%ECCA" with "(g |- eLet y N M : B)%ECCA".
+ *)
+
+
+(* 
+Goal ECCA_has_type Empty (Fst (Pair Tru Fls 
+    (Sig X Bool 
+          (If X Bool (Pi Y Bool Bool))))) Bool.
+Proof.
+eapply aT_Fst with (A:= Bool). eapply aT_Pair.
+  - apply aT_True.
+  - cbv. apply aT_Conv with (A := Bool) (U := (Uni (uType 0))).
+    + apply aT_False.
+    + eapply aT_Conv.
+      * apply aT_If with (e:= Tru) (e1:= Bool) (e2:= (P 1 : Bool -> Bool)%ECCA) (x:= 20) (B:= (Uni (uType 0))) (U:= Uni (uType 1)). 
+        -- apply aT_Ax_Type.
+        -- auto.
+        -- auto.
+        -- cbv. eapply aT_Prod_Type.
+          ++ auto.
+          ++ auto.
+      * apply aT_Ax_Type.
+      * cbn. apply aST_Cong. apply aE_EquivAlpha. apply aeq_id.
+    + apply aST_Cong. apply aE_Equiv with (e:= eBool).
+      * auto.
+      * eauto.
+Qed. *)
