ECCA_reduction.v
@@ -1,0 +1,87 @@
+Require Export ECCA_subst.
+
+
+(*
+=====================================
+=======--Reduction Relation--========
+=====================================
+*)
+
+(* -Step- *)
+Inductive ECCA_RedR : ECCAenv -> ECCAexp -> ECCAexp -> Prop :=
+  | R_ID (g: ECCAenv) (x: atom) (e': ECCAexp) :
+    ECCA_LookupDefR g x e' -> ECCA_RedR g (eId x) e'
+  | R_App (g: ECCAenv) (x: atom) (A body arg: ECCAexp) :
+    ECCA_RedR g (eApp (eAbs x A body) arg) (subst x arg body) (*do anything with env here?*)
+  | R_Fst (g: ECCAenv) (e1 e2 A: ECCAexp) :
+    ECCA_RedR g (eFst (ePair e1 e2 A)) e1
+  | R_Snd (g: ECCAenv) (e1 e2 A: ECCAexp) :
+    ECCA_RedR g (eSnd (ePair e1 e2 A)) e2
+  | R_Let (g: ECCAenv) (x: atom) (e1 e2: ECCAexp) :
+    ECCA_RedR g (eLet x e1 e2) (subst x e1 e2)  (*or here?*)
+(*   | R_IfTru (g: ECCAenv) (e1 e2: ECCAexp) :
+    ECCA_RedR g (eIf eTru e1 e2) e1
+  | R_IfFls (g: ECCAenv) (e1 e2: ECCAexp) :
+    ECCA_RedR g (eIf eFls e1 e2) e2
+  | R_Subst (g: ECCAenv) (e e': ECCAexp) :
+    ECCA_RedR g (eSubst e e e') e' *)
+.
+Hint Constructors ECCA_RedR.
+Bind Scope ECCA_scope with ECCA_RedR.
+
+(* Reflective Transitive Closure of step*)
+Inductive ECCA_RedClosR : ECCAenv -> ECCAexp -> ECCAexp -> Prop :=
+  | R_RedR (g g': ECCAenv) (e e': ECCAexp): (* maybe don't need this one? it follows from refl + trans*)
+      ECCA_RedR g e e' ->
+      ECCA_RedClosR g e e'
+  | R_Refl (g: ECCAenv) (e: ECCAexp):
+      ECCA_RedClosR g e e
+  | R_Trans (g: ECCAenv) (e e' e'': ECCAexp) :
+      ECCA_RedClosR g e e' ->
+      ECCA_RedClosR g e' e'' ->
+      ECCA_RedClosR g e e''
+  | R_CongLet (g: ECCAenv) (e: ECCAexp) (e1 e2: ECCAexp) (x: atom) :
+      ECCA_RedClosR (Def g x e) e1 e2 ->
+      ECCA_RedClosR g (eLet x e e1) (eLet x e e2)
+  | R_CongLam1 (g: ECCAenv) (A: ECCAexp) (A' e e': ECCAexp) (x: atom) :
+      ECCA_RedClosR g A A' ->
+      ECCA_RedClosR (Assum g x A) e e' ->
+      ECCA_RedClosR g (eAbs x A e) (eAbs x A' e')
+  | R_CongPi (g: ECCAenv) (A: ECCAexp) (A' B B': ECCAexp) (x: atom) :
+      ECCA_RedClosR g A A' ->
+      ECCA_RedClosR (Assum g x A) B B' ->
+      ECCA_RedClosR g (ePi x A B) (ePi x A' B')
+  | R_CongSig (g: ECCAenv) (A: ECCAexp) (A' B B': ECCAexp) (x: atom) :
+      ECCA_RedClosR g A A' ->
+      ECCA_RedClosR (Assum g x A) B B' ->
+      ECCA_RedClosR g (eSig x A B) (eSig x A' B')
+  | R_CongPair (g: ECCAenv) (e1 e1' e2 e2' A A': ECCAexp) :
+      ECCA_RedClosR g e1 e1' ->
+      ECCA_RedClosR g e2 e2' ->
+      ECCA_RedClosR g A A'   ->
+      ECCA_RedClosR g (ePair e1 e2 A) (ePair e1' e2' A')
+  | R_CongApp (g: ECCAenv) (e1 e1' e2 e2': ECCAexp) :
+      ECCA_RedClosR g e1 e1' ->
+      ECCA_RedClosR g e2 e2' ->
+      ECCA_RedClosR g (eApp e1 e2) (eApp e1' e2')
+  | R_CongFst (g: ECCAenv) (V V': ECCAexp) :
+      ECCA_RedClosR g V V' ->
+      ECCA_RedClosR g (eFst V) (eFst V')
+  | R_CongSnd (g: ECCAenv) (V V': ECCAexp) :
+      ECCA_RedClosR g V V' ->
+      ECCA_RedClosR g (eSnd V) (eSnd V')
+(*   | R_CongIf (g: ECCAenv) (e e' e1 e1' e2 e2': ECCAexp) :
+      ECCA_RedClosR g e e' ->
+      ECCA_RedClosR g e1 e1' ->
+      ECCA_RedClosR g e2 e2' ->
+      ECCA_RedClosR g (eIf e e1 e2) (eIf e' e1' e2')
+  | R_CongSubst (g: ECCAenv) (e1 e1' e2 e2' e e': ECCAexp):
+      ECCA_RedClosR g e1 e1' ->
+      ECCA_RedClosR g e2 e2' ->
+      ECCA_RedClosR g e e' ->
+      ECCA_RedClosR g (eSubst e1 e2 e) (eSubst e1' e2' e') *)
+.
+Notation "g '|-' e1 '=r>' e2":= (ECCA_RedClosR g e1 e2) (at level 50, e1 at level 99): ECCA_scope.
+(* TODO: rewrite with notation for readability *)
+Hint Constructors ECCA_RedClosR.
+Bind Scope ECCA_scope with ECCA_RedClosR.
