ECCA_subst.v
@@ -1,0 +1,120 @@
+Require Export ECCA_core.
+
+
+(* 
+=====================================
+=======--Substitition--==============
+=====================================
+*)
+
+Fixpoint FV (e: ECCAexp) : atoms :=
+match e with
+  | eId x => singleton x
+  | eUni U => empty
+  | ePi x A B =>  union (FV A) (remove x (FV B))
+  | eAbs x A e => union (FV A) (remove  x (FV e))
+  | eApp  e1 e2 => (union (FV e1) (FV e2))
+  | eLet x e1 e2 => union (FV e1) (remove  x (FV e2))
+  | eSig x A B => (union (FV A) (remove  x (FV B)))
+  | ePair e1 e2 A => (union (union  (FV e1) (FV e2)) (FV A))
+  | eFst e => (FV e)
+  | eSnd e => (FV e)
+(*   | eIf e e1 e2 => (union (union  (FV e) (FV e1)) (FV e2)) *)
+  | _ => empty
+end.
+
+(*Let's get nominal!*)
+
+Fixpoint swap (x:atom) (y:atom) (t:ECCAexp) : ECCAexp :=
+  match t with
+  | eId z     => eId (swap_var x y z)
+  | eAbs z A t1  => eAbs (swap_var x y z) (swap x y A) (swap x y t1)
+  | eApp t1 t2 => eApp (swap x y t1) (swap x y t2)
+  | ePi x' A B => ePi (swap_var x y x') (swap x y A) (swap x y B)
+  | eLet x' e1 e2 => eLet (swap_var x y x') (swap x y e1) (swap x y e2)
+  | eSig x' A B => eSig (swap_var x y x') (swap x y A) (swap x y B)
+  | ePair e1 e2 A => ePair (swap x y e1) (swap x y e2) (swap x y A)
+  | eFst e => (eFst (swap x y e))
+  | eSnd e => (eSnd (swap x y e))
+(*   | eIf e e1 e2 => (eIf (swap x y e) (swap x y e1) (swap x y e2)) *)
+  | _ => t
+  end.
+
+Fixpoint ECCAsize (e: ECCAexp) : nat :=
+  match e with
+  | eId _ => 1
+  | eUni _ => 1
+  | ePi _ A B => 1 + (ECCAsize A) + (ECCAsize B)
+  | eAbs _ A e => 1 + (ECCAsize A) + (ECCAsize e)
+  | eApp e1 e2 => 1 + (ECCAsize e1) + (ECCAsize e2)
+  | eLet _ e1 e2 => 1 + (ECCAsize e1) + (ECCAsize e2)
+  | eSig _ A B => 1 + (ECCAsize A) + (ECCAsize B)
+  | ePair e1 e2 A => 1 + (ECCAsize e1) + (ECCAsize e2) + (ECCAsize A)
+  | eFst e => 1 + (ECCAsize e)
+  | eSnd e => 1 + (ECCAsize e)
+(*   | eIf e e1 e2 => 1 + (ECCAsize e) + (ECCAsize e1) + (ECCAsize e2) *)
+(*   | eSubst a b c => 1 + (ECCAsize a) + (ECCAsize b) + (ECCAsize c) *)
+  | _ => 1
+end.
+
+Lemma ECCAsize_non_zero : forall e, 0 < ECCAsize e.
+Proof.
+  induction e; simpl; omega.
+Qed.
+
+Lemma swap_size_eq : forall x y t,
+    ECCAsize (swap x y t) = ECCAsize t.
+Proof.
+  induction t; simpl; auto.
+Qed.
+
+(* If there are free variables in the substitute,
+   and if the term being substituted in binds one of them,
+   then we need to perform an alpha conversion of the term being substituted in
+   that avoids capturing any free variables in the substitute or in the body
+   of the term being substituted in. *)
+Require Import Recdef.
+
+Function substWork (x: atom) (arg body: ECCAexp) {measure ECCAsize body}:=
+if (AtomSetImpl.mem x (FV body)) then 
+  match body with
+    | eId x' => if (x == x') then arg else body
+    | eAbs x' A e =>
+        if (x == x')
+          then (eAbs x' (substWork x arg A) e)
+          else let (xnew,_) := atom_fresh (union (FV arg) (FV e)) in
+                      (eAbs xnew (substWork x arg A) (substWork x arg (swap x' xnew e)))
+    | ePi x' A B =>
+        if (x == x')
+          then (ePi x' (substWork x arg A) B)
+          else let (xnew,_) := atom_fresh (union (FV arg) (FV B)) in
+                  (ePi xnew (substWork x arg A) (substWork x arg (swap x' xnew B)))
+    | eLet x' A B =>
+        if (x == x')
+          then (eLet x' (substWork x arg A) B)
+          else let (xnew,_) := atom_fresh (union (FV arg) (FV B)) in
+                  (eLet xnew (substWork x arg A) (substWork x arg (swap x' xnew B)))
+    | eSig x' A B =>
+        if (x == x')
+          then (eSig x' (substWork x arg A) B)
+          else let (xnew,_) := atom_fresh (union (FV arg) (FV B)) in
+                  (eSig xnew (substWork x arg A) (substWork x arg (swap x' xnew B)))
+    | eApp e1 e2 => (eApp (substWork x arg e1) (substWork x arg e2))
+    | ePair e1 e2 A => (ePair (substWork x arg e1) (substWork x arg e2) (substWork x arg A))
+    | eFst e => (eFst (substWork x arg e))
+    | eSnd e => (eSnd (substWork x arg e))
+  (*   | eIf e e1 e2 => (eIf (substWork x arg e FVInArg) (substWork x arg e1 FVInArg) (substWork x arg e2 FVInArg)) *)
+    | _ => body
+  (*   | eSubst a b c => eSubst (substWork x arg a FVInArg) (substWork x arg b FVInArg) (substWork x arg c FVInArg) (**) *)
+  end
+else body
+.
+Proof.
+1-19: try (Tactics.program_simpl; cbn; omega).
+1-4: try (Tactics.program_simpl; cbn; rewrite -> swap_size_eq; omega).
+Qed.
+
+Definition subst (x: atom) (arg body: ECCAexp):= substWork x arg body.
+Search "substWork_eq".
+
+Notation "b '[' a '/' x ']'":= (subst x a b) (at level 50): ECCA_scope. 
