ECCA_subst_lemmas.v
@@ -1,0 +1,83 @@
+Require Export ECCA_subst.
+
+Lemma notin_fv_equivariance : forall x0 x y t ,
+  x0 `notin` FV t ->
+  swap_var x y x0  `notin` FV (swap x y t).
+Proof.
+  induction t; intros; simpl in *.
+  1-13: unfold swap_var in *; auto; default_simp.  
+Qed.
+Hint Resolve notin_fv_equivariance.
+
+Lemma notin_fv_equivariance_easy (x y: atom) (b1 b2: ECCAexp):
+(x `notin` FV b2 ->
+y `notin` FV (swap y x b2))%ECCA.
+Proof. intros. cut (y = (swap_var y x x)).
++ intros. rewrite H0 at 1. apply notin_fv_equivariance. assumption.
++ unfold swap_var. default_simp.
+Qed.
+
+Lemma in_fv_equivariance : forall x y x0 t,
+  x0 `in` FV t ->
+  swap_var x y x0 `in` FV (swap x y t).
+Proof.
+  (* ADMITTED *)
+  induction t; intros; simpl in *.
+  all: try (unfold swap_var; default_simp; fsetdec).
+  all: destruct (AtomSetImpl.union_1 H); unfold swap_var in *; default_simp; fsetdec.
+Qed. (* ADMITTED *)
+Hint Resolve in_fv_equivariance.
+
+Lemma swap_involutive : forall t x y,
+    swap x y (swap x y t) = t.
+Proof.
+  (* ADMITTED *)
+  induction t;  simpl; unfold swap_var; default_simp.
+Qed.
+Hint Resolve swap_involutive.
+
+Lemma swap_id : forall n x,
+    swap x x n = n.
+Proof.
+  induction n; simpl; unfold swap_var;  default_simp.
+Qed.
+Hint Resolve swap_id.
+
+Lemma swap_symmetric : forall t x y,
+    swap x y t = swap y x t.
+Proof.
+  induction t;  simpl; unfold swap_var; default_simp.
+Qed. 
+Hint Resolve swap_symmetric.
+
+Lemma swap_var_equivariance : forall v x y z w,
+    swap_var x y (swap_var z w v) =
+    swap_var (swap_var x y z) (swap_var x y w) (swap_var x y v).
+Proof.
+  unfold swap_var; default_simp.
+Qed.
+Hint Resolve swap_var_equivariance.
+
+Lemma swap_equivariance : forall t x y z w,
+    swap x y (swap z w t) = swap (swap_var x y z) (swap_var x y w) (swap x y t).
+Proof.
+  induction t; intros; simpl; try rewrite swap_var_equivariance; try auto.
+  1,2,3,5: rewrite swap_var_equivariance; rewrite IHt1; rewrite IHt2; auto.
+  all: default_simp.
+Qed.
+Hint Resolve swap_equivariance.
+
+Lemma subst_distributes_over_app (y: atom) (A B1 B2: ECCAexp) :
+ subst y A (eApp B1 B2) = eApp (subst y A B1) (subst y A B2).
+Proof.
+- rewrite substWork_equation. case_eq (AtomSetImpl.mem y (FV (eApp B1 B2))).
+  + intros. auto.
+  + intros. default_simp.
+    * cut (AtomSetImpl.mem y (FV B1) = false).
+      -- intros. rewrite substWork_equation. rewrite H0. reflexivity. 
+      -- rewrite <- not_mem_iff. rewrite <- not_mem_iff in H. fsetdec.
+    * cut (AtomSetImpl.mem y (FV B2) = false).
+      -- intros. rewrite substWork_equation. rewrite H0. reflexivity. 
+      -- rewrite <- not_mem_iff. rewrite <- not_mem_iff in H. fsetdec.
+ Qed.
+Hint Resolve subst_distributes_over_app.
