ECCA_typing.v
@@ -1,0 +1,157 @@
+Require Export ECCA_equiv.
+
+(*
+================================
+=======--Type System--==========
+================================
+*)
+
+(* TODO: Add notation for subtypes. *)
+Inductive ECCA_sub_type: ECCAenv -> ECCAexp -> ECCAexp -> Prop :=
+| aST_Cong (g: ECCAenv) (A B: ECCAexp) :
+  ECCA_Equiv g A B ->
+  ECCA_sub_type g A B
+| aST_Cum (g: ECCAenv) (i: nat) :
+  ECCA_sub_type g (eUni (uType i)) (eUni (uType (S i)))
+| aST_Pi (g: ECCAenv) (A1 A2 B1 B2: ECCAexp) (x1 x2: atom) :
+  (ECCA_Equiv g A1 A2) ->
+  (ECCA_sub_type (Assum g x1 A2) B1 (subst x2 (eId x1) B2)) -> (* eId x1 ?*)
+  (ECCA_sub_type g (ePi x1 A1 B1) (ePi x2 A2 B2))
+.
+Hint Constructors ECCA_sub_type.
+
+Reserved Notation "g '|-' a ':' b" (at level 50, a at level 99).
+Inductive ECCA_has_type: ECCAenv -> ECCAexp -> ECCAexp -> Prop :=
+| aT_Ax_Prop (g: ECCAenv) :
+  (g |- (eUni uProp) : (eUni (uType 0)))
+| aT_Ax_Type (g: ECCAenv) (i: nat) :
+  (g |- (eUni (uType i)) : (eUni (uType (S i))))
+| aT_Var (g: ECCAenv) (x: atom) (A: ECCAexp) :
+  (ECCA_LookupTypeR g x A) -> (* this needs adjustment *)
+  (g |- (eId x) : A)
+| aT_Bool (g: ECCAenv):
+  (g |- (eBool) : (eUni (uType 0)))
+| aT_True (g: ECCAenv):
+  (g |- (eTru) : (eBool))
+| aT_False (g: ECCAenv):
+  (g |- (eFls) : (eBool)) 
+| aT_Sig (g: ECCAenv) (x: atom) (A B: ECCAexp) (i: nat) :
+  (g |- A : (eUni (uType i))) ->
+  (ECCA_has_type (Assum g x A) B (eUni (uType i))) ->
+  (g |- (eSig x A B) : (eUni (uType i)))
+| aT_Pair (g: ECCAenv) (v1 v2: ECCAexp) (A B: ECCAexp) (x: atom) :
+  (g |- v1 : A) ->
+  (g |- v2 : (subst x v1 B)) ->
+  (g |- (ePair v1 v2 (eSig x A B)) : (eSig x A B))
+| aT_Prod_Prop (g: ECCAenv) (x: atom) (A B: ECCAexp) (i: nat):
+  (g |- A : (eUni (uType i))) ->
+  (ECCA_has_type (Assum g x A) B (eUni (uProp))) ->
+  (g |- (ePi x A B) : (eUni (uProp)))
+| aT_Prod_Type (g: ECCAenv) (x: atom) (A B: ECCAexp) (i: nat):
+  (g |- A : (eUni (uType i))) ->
+  (ECCA_has_type (Assum g x A) B (eUni (uType i))) ->
+  (g |- (ePi x A B) : (eUni (uType i)))
+| aT_Lam (g: ECCAenv) (x: atom) (A e B: ECCAexp) :
+  (ECCA_has_type (Assum g x A) e B) ->
+  (g |- (eAbs x A e) : (ePi x A B))
+(* ECCA_has_type: ECCAenv -> ECCAconf -> ECCAconf -> Prop := *)
+| aT_Let (g: ECCAenv) (n m A B: ECCAexp) (x: atom):
+  (g |- n : A) ->
+(*should this be (def(assum(g))) or (assum(def(g)))*)
+  (ECCA_has_type (Assum (Def g x n) x A) m B) ->
+  (g |- (eLet x n m) : (subst x n B))
+(* | aT_If (g: ECCAenv) (B U e1 e2: ECCAexp) (e: ECCAexp) (x: atom):
+  ECCA_has_type (Assum g x eBool) B U -> 
+  g |- e : eBool ->
+  ECCA_has_type (Eq g e eTru) e1 (subst x eTru B) ->
+  ECCA_has_type (Eq g e eFls) e2 (subst x eFls B) -> 
+  g |- (eIf e e1 e2) : (subst x e B) *)
+| aT_Conv (g: ECCAenv) (e A B U: ECCAexp) :
+  (g |- e : A) ->
+  (g |- B : U) ->
+  (ECCA_sub_type g A B) ->
+  (g |- e : B)
+(* ECCA_has_type: ECCAenv -> ECCAcomp -> ECCAconf -> Prop := *)
+| aT_App (g: ECCAenv) (x: atom) (e e': ECCAexp) (A' B: ECCAexp) :
+  (g |- e : (ePi x A' B)) ->
+  (g |- e' : A') ->
+  (g |- (eApp e e') : (subst x e B))
+| aT_Fst (g: ECCAenv) (e: ECCAexp) (A B: ECCAexp) (x: atom) :
+  (g |- e: (eSig x A B)) ->
+  (g |- (eFst e): A)
+| aT_Snd (g: ECCAenv) (e: ECCAexp) (A B: ECCAexp) (x: atom) :
+  (g |- e: (eSig x A B)) ->
+  (g |- (eSnd e): (subst x (eFst e) B)) 
+(* | aT_Subst (x: atom) (g: ECCAenv) (A B U: ECCAexp) (e e1 e2: ECCAexp):
+  (ECCA_has_type (Assum g x A) B U) ->
+  g |- e1: A -> 
+  g |- e2: A ->
+  g |- e: (subst x e1 B) ->
+  ECCA_LookupEqR g e1 e2 ->
+  g |- (eSubst e1 e2 e): (subst x e2 B)  *)
+where "g '|-' a ':' b" := (ECCA_has_type g a b) : ECCA_scope
+.
+Check (Empty |- eTru : eBool)%ECCA.
+
+Hint Constructors ECCA_has_type.
+
+Goal ECCA_has_type Empty eBool (eUni (uType 0)).
+Proof.
+intros. apply aT_Bool. Qed.
+
+Hint Resolve substWork_equation.
+
+Goal ECCA_has_type Empty (ePair eTru eBool (eSig X eBool (eUni (uType 0)))) (eSig X eBool (eUni (uType 0))).
+Proof.
+intros. apply aT_Pair. 
+- apply aT_True.
+- rewrite substWork_equation. destruct AtomSetImpl.mem; apply aT_Bool.
+Qed.
+
+(*===========================
+  ==--Continuation Typing--==
+  ===========================*)
+
+(* TODO: incomplete *)
+
+Inductive ECCAcont: Type :=
+  | Hole
+  | LetHole (x: atom) (E: ECCAexp)
+.
+Hint Constructors ECCAcont.
+Bind Scope ECCA_scope with ECCAcont.
+
+Notation "'[]'" := (Hole) (at level 50) : ECCA_scope.
+Definition aHole := []%ECCA.
+Notation "'LET' x ':=' '[]' 'in' B" := (LetHole x B) (at level 50) : ECCA_scope.
+Definition example_aLetHole := (LET X := [] in (eId X))%ECCA.
+
+Inductive ECCAconttype: Type :=
+  | Cont (M: ECCAexp) (A: ECCAexp) (B: ECCAexp)
+.
+Hint Constructors ECCAconttype.
+(* TODO: Add notation for cont type  *)
+
+
+
+Inductive ECCA_cont_has_type: ECCAenv -> ECCAcont -> ECCAconttype -> Prop :=
+  | aK_Empty (M: ECCAexp) (g: ECCAenv) (A: ECCAexp):
+    ECCA_cont_has_type g Hole (Cont M A A)
+  | aK_Bind (g: ECCAenv) (y: atom) (M: ECCAexp) (M' A B: ECCAexp):
+    ECCA_has_type g M' A ->
+    ECCA_has_type (Assum (Def g y M') y A) M B ->
+    y `notin` FV B ->  (*Prove as a lemma later*)
+    ECCA_cont_has_type g (LetHole y M) (Cont M' A B)
+.
+
+Hint Constructors ECCA_cont_has_type.
+
+Definition fill_hole (e: ECCAexp) (K: ECCAcont): ECCAexp :=
+  match K with
+    | Hole => e
+    | LetHole x B => eLet x e B
+end.
+
+Lemma fill_with_hole_is_id (e: ECCAexp): fill_hole e Hole = e.
+Proof.
+eauto. Qed.
