outdated/ECCtoECCAold.v
@@ -1,0 +1,1103 @@
+
+(*From Coq Require Import Strings.String.
+From Coq Require Import Strings.Ascii.
+From Coq Require Import Init.Datatypes.*)
+Require Import Omega.
+Require Import Coq.Lists.ListSet.
+Require Import Coq.Init.Nat.
+Require Import Coq.Arith.EqNat.
+Require Import Arith.
+Require Import Coq.Program.Wf.
+Open Scope list.
+
+Definition atom:= nat.
+Definition atoms := set atom.
+Definition empty : atoms := empty_set atom.
+Definition singleton (x : atom) := x :: nil.
+
+Definition union := set_union Nat.eq_dec.
+Definition remove := set_remove Nat.eq_dec.
+Definition add := set_add Nat.eq_dec.
+Definition mem := set_mem Nat.eq_dec.
+
+Definition fresh (ns: atoms): atom :=
+(set_fold_left max ns 0) + 1
+.
+
+Definition X: atom := (fresh nil).
+Definition Y: atom := (fresh (X :: nil)).
+Definition Z: atom := (fresh (X :: Y :: nil)).
+
+
+(* Module ECC. *)
+
+(* -=ECC Definition=- *)
+
+Inductive ECCuni: Type :=
+  | uProp
+  | uType (i: nat)
+.
+
+Inductive ECCexp: Type :=
+  | eId (x: atom)
+  | eUni (U: ECCuni)
+  | ePi (x: atom) (A B: ECCexp)
+  | eAbs (x: atom) (A e: ECCexp)
+  | eApp  (e1 e2: ECCexp)
+  | eLet (x: atom) (e1 e2: ECCexp)
+  | eSig (x: atom) (A B: ECCexp)
+  | ePair (e1 e2 A: ECCexp)
+  | eFst (e: ECCexp)
+  | eSnd (e: ECCexp)
+  | eIf (e e1 e2: ECCexp)
+  | eTru
+  | eFls
+  | eBool
+.
+
+Inductive ECCenv: Type :=
+  | gEmpty
+  | gAssum (g: ECCenv) (x: atom) (A: ECCexp)
+  | gDef (g: ECCenv) (x: atom) (e: ECCexp)
+.
+
+Fixpoint ECCsize (e: ECCexp) : nat :=
+  match e with
+  | eId _ => 1
+  | eUni _ => 1
+  | ePi _ A B => 1 + (ECCsize A) + (ECCsize B)
+  | eAbs _ A e => 1 + (ECCsize A) + (ECCsize e)
+  | eApp e1 e2 => 1 + (ECCsize e1) + (ECCsize e2)
+  | eLet _ e1 e2 => 1 + (ECCsize e1) + (ECCsize e2)
+  | eSig _ A B => 1 + (ECCsize A) + (ECCsize B)
+  | ePair e1 e2 A => 1 + (ECCsize e1) + (ECCsize e2) + (ECCsize A)
+  | eFst e => 1 + (ECCsize e)
+  | eSnd e => 1 + (ECCsize e)
+  | eIf e e1 e2 => 1 + (ECCsize e) + (ECCsize e1) + (ECCsize e2)
+  | eTru => 1
+  | eFls => 1
+  | eBool => 1
+end.
+
+Hint Constructors ECCuni.
+Hint Constructors ECCexp.
+Hint Constructors ECCenv.
+
+Lemma ECCsize_non_zero : forall e, 0 < ECCsize e.
+Proof.
+  induction e; simpl; omega.
+Qed.
+
+(* -=ECC Evaluation=- *)
+
+(* -Lookup- *)
+
+Inductive ECC_LookupTypeR : ECCenv -> atom -> ECCexp -> Prop:=
+  | LT_gFirst (g': ECCenv) (x: atom) (A: ECCexp):
+    ECC_LookupTypeR (gAssum g' x A) x A
+  | LT_AssumRest (g: ECCenv) (x x': atom) (A a': ECCexp):
+    ECC_LookupTypeR g x A ->
+    (x <> x') ->
+    (ECC_LookupTypeR (gAssum g x' a') x A)
+  | LT_DefRest (g: ECCenv) (x x': atom) (A a': ECCexp):
+    ECC_LookupTypeR g x A ->
+(*     (x <> x') -> *)
+    (ECC_LookupTypeR (gDef g x' a') x A)
+.
+
+Inductive ECC_LookupDefR : ECCenv -> atom -> ECCexp -> Prop:=
+  | LD_gFirst (g': ECCenv) (x: atom) (e A: ECCexp):
+    ECC_LookupDefR (gAssum (gDef g' x e) x A) x e
+  | LD_AssumRest (g: ECCenv) (x x': atom) (e a': ECCexp):
+    ECC_LookupDefR g x e ->
+    (x <> x') ->
+    (ECC_LookupDefR (gAssum g x' a') x e)
+  | LD_DefRest (g: ECCenv) (x x': atom) (e e': ECCexp):
+    ECC_LookupDefR g x e ->
+    (x <> x') ->
+    (ECC_LookupDefR (gDef g x' e') x e)
+.
+(* Q: what if looking up a type and get a value first, or vice versa? *)
+
+Hint Constructors ECC_LookupTypeR.
+
+Example ECC_LookupFirstExample:
+ECC_LookupTypeR (gAssum gEmpty X eTru) X eTru.
+Proof.
+  auto.
+Qed.
+
+Example ECC_LookupRestExample:
+X <> Y -> ECC_LookupTypeR (gAssum (gAssum gEmpty X eTru) Y eFls) X eTru.
+Proof.
+  auto.  (* WOW!*)
+Qed.
+
+Fixpoint ECC_LookupType (g: ECCenv) (x: atom): option ECCexp :=
+match g with
+  | gEmpty => None
+  | gAssum g' x' A => if (x' =? x) then Some A else (ECC_LookupType g' x)
+  | gDef g' x' e => (ECC_LookupType g' x)
+end.
+
+Fixpoint ECC_LookupDef (g: ECCenv) (x: atom): option ECCexp :=
+match g with
+  | gEmpty => None
+  | gAssum g' x' A => if (x' =? x) then match g' with
+      | gEmpty => None
+      | gAssum g'' x'' A => None
+      | gDef g' x'' e => if (x'' =? x) then Some e else None
+      end      
+      else (ECC_LookupDef g' x)
+  | gDef g' x' e => if (x' =? x) then None else (ECC_LookupDef g' x)
+end.
+
+Lemma ECC_EmptyImpliesNothing : forall (x: atom) (A: ECCexp), ECC_LookupTypeR gEmpty x A -> False.
+Proof.
+intros. inversion H.
+Qed.
+
+Lemma ECC_LookupTypeReflects (g: ECCenv) (x: atom) (A: ECCexp) : ECC_LookupTypeR g x A <-> (ECC_LookupType g x) = Some A.
+Proof.
+intros. split.
+ - intros. induction H.
+  + cbn. rewrite <- beq_nat_refl. reflexivity.
+  + cbn. cut (x' =? x = false).
+    * intros. rewrite H1. apply IHECC_LookupTypeR.
+    * apply Nat.eqb_neq. auto.
+  + cbn. apply IHECC_LookupTypeR.
+ - intros. induction g.
+  + discriminate.
+  + inversion H. destruct (x0 =? x) eqn:eq.
+    * inversion H1. apply Nat.eqb_eq in eq. rewrite eq. apply LT_gFirst.
+    * apply LT_AssumRest.
+      -- apply IHg. apply H1.
+      -- apply Nat.eqb_neq in eq. auto.
+  + apply LT_DefRest.
+    * apply IHg. apply H.
+Qed.
+
+Lemma ECC_LookupDefReflects (g: ECCenv) (x: atom) (A: ECCexp) : ECC_LookupDefR g x A <-> (ECC_LookupDef g x) = Some A.
+Proof.
+intros. split.
+ - intros. induction H.
+  + cbn. rewrite <- beq_nat_refl. reflexivity.
+  + cbn. cut (x' =? x = false).
+    * intros. rewrite H1. apply IHECC_LookupDefR.
+    * apply Nat.eqb_neq. auto.
+  + cbn. cut (x' =? x = false). 
+    * intros. rewrite H1. apply IHECC_LookupDefR.
+    * apply Nat.eqb_neq. auto.
+ - intros. induction g.
+  + discriminate.
+  + inversion H. destruct (x0 =? x) eqn:eq.
+    *  destruct g eqn:eq2.
+      -- discriminate.
+      -- discriminate.
+      -- apply Nat.eqb_eq in eq. rewrite eq. destruct (x1 =? x) eqn:eq3.
+        ++ inversion H1. apply Nat.eqb_eq in eq3. rewrite eq3. apply LD_gFirst.
+        ++ discriminate.
+   * apply LD_AssumRest.
+     -- apply IHg. apply H1.
+     -- apply Nat.eqb_neq in eq. auto.
+  + inversion H. destruct (x0 =? x) eqn:eq.
+    * discriminate.
+    * apply LD_DefRest.
+      -- apply IHg. apply H1.
+      -- apply Nat.eqb_neq in eq. auto.
+Qed.
+
+(* Substitution *)
+
+
+Fixpoint FV (e: ECCexp) : atoms :=
+match e with
+  | eId x => singleton x
+  | eUni U => empty
+  | ePi x A B =>  union (FV A) (remove x (FV B))
+  | eAbs x A e => union (FV A) (remove  x (FV e))
+  | eApp  e1 e2 => (union (FV e1) (FV e2))
+  | eLet x e1 e2 => (union (FV e1) (FV e2))
+  | eSig x A B => (union (FV A) (remove  x (FV B)))
+  | ePair e1 e2 A => (union (union  (FV e1) (FV e2)) (FV A))
+  | eFst e => (FV e)
+  | eSnd e => (FV e)
+  | eIf e e1 e2 => (union (union  (FV e) (FV e1)) (FV e2))
+  | eTru => empty
+  | eFls => empty
+  | eBool => empty
+end.
+
+(*Let's get nominal!*)
+
+Definition swap_var (x:atom) (y:atom) (z:atom) :=
+  if (z =? x) then y else if (z =? y) then x else z.
+
+Fixpoint swap (x:atom) (y:atom) (t:ECCexp) : ECCexp :=
+  match t with
+  | eId z     => eId (swap_var x y z)
+  | eAbs z A t1  => eAbs (swap_var x y z) (swap x y A) (swap x y t1)
+  | eApp t1 t2 => eApp (swap x y t1) (swap x y t2)
+  | ePi x' A B => ePi (swap_var x y x') (swap x y A) (swap x y B)
+  | eLet x' e1 e2 => eLet (swap_var x y x') (swap x y e1) (swap x y e2)
+  | eSig x' A B => eSig (swap_var x y x') (swap x y A) (swap x y B)
+  | ePair e1 e2 A => ePair (swap x y e1) (swap x y e2) (swap x y A)
+  | eFst e => (eFst (swap x y e))
+  | eSnd e => (eSnd (swap x y e))
+  | eIf e e1 e2 => (eIf (swap x y e) (swap x y e1) (swap x y e2))
+  | _ => t
+  end.
+
+Lemma swap_size_eq : forall x y t,
+    ECCsize (swap x y t) = ECCsize t.
+Proof.
+  induction t; simpl; auto.
+Qed.
+
+
+(* If there are free variables in the substitute,
+   and if the term being substituted in binds one of them,
+   then we need to perform an alpha conversion of the term being substituted in
+   that avoids capturing any free variables in the substitute or in the body
+   of the term being substituted in. *)
+
+Program Fixpoint substWork (x: atom) (arg body: ECCexp) (FVInArg: atoms) {measure (ECCsize body)}:=
+match body with
+  | eId x' => if (x =? x') then arg else body
+  | eAbs x' A e =>
+      if (x =? x')
+        then (eAbs x' (substWork x arg A FVInArg) e)
+        else let xnew := fresh (union FVInArg (FV e)) in
+                    (eAbs xnew (substWork x arg A FVInArg) (substWork x arg (swap x' xnew e) FVInArg))
+  | ePi x' A B =>
+      if (x =? x')
+        then (ePi x' (substWork x arg A FVInArg) B)
+        else let xnew := fresh (union FVInArg (FV B)) in
+                (ePi xnew (substWork x arg A FVInArg) (substWork x arg (swap x' xnew B) FVInArg))
+  | eLet x' A B =>
+      if (x =? x')
+        then (eLet x' (substWork x arg A FVInArg) B)
+        else let xnew := fresh (union FVInArg (FV B)) in
+                (eLet xnew (substWork x arg A FVInArg) (substWork x arg (swap x' xnew B) FVInArg))
+  | eSig x' A B =>
+      if (x =? x')
+        then (eSig x' (substWork x arg A FVInArg) B)
+        else let xnew := fresh (union FVInArg (FV B)) in
+                (eSig xnew (substWork x arg A FVInArg) (substWork x arg (swap x' xnew B) FVInArg))
+  | eApp e1 e2 => (eApp (substWork x arg e1 FVInArg) (substWork x arg e2 FVInArg))
+  | eUni U => body
+  | ePair e1 e2 A => (ePair (substWork x arg e1 FVInArg) (substWork x arg e2 FVInArg) (substWork x arg A FVInArg))
+  | eFst e => (eFst (substWork x arg e FVInArg))
+  | eSnd e => (eSnd (substWork x arg e FVInArg))
+  | eIf e e1 e2 => (eIf (substWork x arg e FVInArg) (substWork x arg e1 FVInArg) (substWork x arg e2 FVInArg))
+  | eTru => eTru
+  | eFls => eFls
+  | eBool => eBool
+end.
+Obligations.
+Solve Obligations with (Tactics.program_simpl; cbn; omega).
+Solve Obligations with (Tactics.program_simpl; cbn; rewrite -> swap_size_eq; omega).
+
+Definition subst (x: atom) (arg body: ECCexp):= substWork x arg body (FV arg).
+
+Inductive ECC_Aeq : ECCexp -> ECCexp -> Prop :=
+  | aeq_id (e: ECCexp):
+    ECC_Aeq e e
+  | aeq_var (x: atom):
+     ECC_Aeq (eId x) (eId x)
+  | aeq_abs_same (x: atom) (t1 t2 b1 b2: ECCexp):
+     ECC_Aeq t1 t2 -> 
+     ECC_Aeq b1 b2 ->
+     ECC_Aeq (eAbs x t1 b1) (eAbs x t2 b2)
+  | aeq_abs_diff (x y: atom) (t1 t2 b1 b2: ECCexp):
+     x <> y ->
+     (mem x (FV b2)) = false ->
+     ECC_Aeq b1 (swap y x b2) ->
+     ECC_Aeq t1 t2 ->
+     ECC_Aeq (eAbs x t1 b1) (eAbs y t2 b2)
+  | aeq_pi_same (x: atom) (t1 t2 b1 b2: ECCexp):
+     ECC_Aeq t1 t2 -> 
+     ECC_Aeq b1 b2 ->
+     ECC_Aeq (ePi x t1 b1) (ePi x t2 b2)
+  | aeq_pi_diff (x y: atom) (t1 t2 b1 b2: ECCexp):
+     x <> y ->
+     (mem x (FV b2)) = false ->
+     ECC_Aeq b1 (swap y x b2) ->
+     ECC_Aeq t1 t2 ->
+     ECC_Aeq (ePi x t1 b1) (ePi y t2 b2)
+  | aeq_let_same (x: atom) (t1 t2 b1 b2: ECCexp):
+     ECC_Aeq t1 t2 -> 
+     ECC_Aeq b1 b2 ->
+     ECC_Aeq (eLet x t1 b1) (eLet x t2 b2)
+  | aeq_let_diff (x y: atom) (t1 t2 b1 b2: ECCexp):
+     x <> y ->
+     (mem x (FV b2)) = false ->
+     ECC_Aeq b1 (swap y x b2) ->
+     ECC_Aeq t1 t2 ->
+     ECC_Aeq (eLet x t1 b1) (eLet y t2 b2)
+  | aeq_sig_same (x: atom) (t1 t2 b1 b2: ECCexp):
+     ECC_Aeq t1 t2 -> 
+     ECC_Aeq b1 b2 ->
+     ECC_Aeq (eSig x t1 b1) (eSig x t2 b2)
+  | aeq_sig_diff (x y: atom) (t1 t2 b1 b2: ECCexp):
+     x <> y ->
+     (mem x (FV b2)) = false ->
+     ECC_Aeq b1 (swap y x b2) ->
+     ECC_Aeq t1 t2 ->
+     ECC_Aeq (eSig x t1 b1) (eSig y t2 b2)
+  | aeq_app (t1 t2 t1' t2': ECCexp):
+     ECC_Aeq t1 t1' -> ECC_Aeq t2 t2' ->
+     ECC_Aeq (eApp t1 t2) (eApp t1' t2')
+  | aeq_pair (t1 t2 t1' t2' A A': ECCexp):
+     ECC_Aeq t1 t1' -> ECC_Aeq t2 t2' ->
+     ECC_Aeq A A' ->
+     ECC_Aeq (ePair t1 t2 A) (ePair t1' t2' A')
+  | aeq_eFst (e e': ECCexp):
+     ECC_Aeq e e' ->
+     ECC_Aeq (eFst e) (eFst e')
+  | aeq_eSnd (e e': ECCexp):
+     ECC_Aeq e e' ->
+     ECC_Aeq (eSnd e) (eSnd e')
+  | aeq_if (e1 e2 e3 e1' e2' e3': ECCexp):
+     ECC_Aeq e1 e1' ->
+     ECC_Aeq e2 e2' ->
+     ECC_Aeq e3 e3' ->
+     ECC_Aeq (eIf e1 e2 e3) (eIf e1' e2' e3').
+
+Hint Constructors ECC_Aeq.
+
+Timeout 30 Compute substWork X (eTru) (eId X) (FV eTru). 
+Compute substWork X (eTru) (eAbs Y (eBool) (eId X)) (FV eTru).
+Compute substWork X (eTru) (eAbs X (eId X) (eId X)) (FV eTru).
+Eval vm_compute in substWork X (eTru) (eAbs X (eId X) (eId X)) (FV eTru).
+
+
+(* -Step- *)
+Inductive ECC_RedR : ECCenv -> ECCexp -> ECCexp -> Prop :=
+  | R_ID (g: ECCenv) (x: atom) (e': ECCexp) :
+    ECC_LookupDefR g x e' -> ECC_RedR g (eId x) e'
+  | R_App (g: ECCenv) (x: atom) (A body arg: ECCexp) :
+    ECC_RedR g (eApp (eAbs x A body) arg) (subst x arg body) (*do anything with env here?*)
+  | R_Fst (g: ECCenv) (e1 e2 A: ECCexp) :
+    ECC_RedR g (eFst (ePair e1 e2 A)) e1
+  | R_Snd (g: ECCenv) (e1 e2 A: ECCexp) :
+    ECC_RedR g (eSnd (ePair e1 e2 A)) e2
+  | R_Let (g: ECCenv) (x: atom) (e1 e2: ECCexp) :
+    ECC_RedR g (eLet x e1 e2) (subst x e1 e2)  (*or here?*)
+  | R_IfTru (g: ECCenv) (e1 e2: ECCexp) :
+    ECC_RedR g (eIf eTru e1 e2) e1
+  | R_IfFls (g: ECCenv) (e1 e2: ECCexp) :
+    ECC_RedR g (eIf eFls e1 e2) e2
+.
+
+Hint Constructors ECC_RedR.
+
+(* Reflective Transitive Closure of step*)
+Inductive ECC_RedClosR : ECCenv -> ECCexp -> ECCexp -> Prop :=
+  (*| R_RedR (g g': ECCenv) (e e': ECCexp): (* maybe don't need this one? it follows from refl + trans*)
+      ECC_RedR g e e' ->
+      ECC_RedClosR g e e'*)
+  | R_Refl (g: ECCenv) (e: ECCexp):
+      ECC_RedClosR g e e
+  | R_Trans (g: ECCenv) (e e' e'': ECCexp) :
+      ECC_RedR g e e' ->
+      ECC_RedClosR g e' e'' ->
+      ECC_RedClosR g e e''
+  | R_CongLet (g: ECCenv) (e e1 e2: ECCexp) (x: atom) :
+      ECC_RedClosR (gDef g x e) e1 e2 ->
+      ECC_RedClosR g (eLet x e e1) (eLet x e e2)
+  | R_CongLam1 (g: ECCenv) (A A' e e': ECCexp) (x: atom) :
+      ECC_RedClosR g A A' ->
+      ECC_RedClosR (gAssum g x A) e e' ->
+      ECC_RedClosR g (eAbs x A e) (eAbs x A' e')
+  | R_CongPi (g: ECCenv) (A A' B B': ECCexp) (x: atom) :
+      ECC_RedClosR g A A' ->
+      ECC_RedClosR (gAssum g x A) B B' ->
+      ECC_RedClosR g (ePi x A B) (ePi x A' B')
+  | R_CongSig (g: ECCenv) (A A' B B': ECCexp) (x: atom) :
+      ECC_RedClosR g A A' ->
+      ECC_RedClosR (gAssum g x A) B B' ->
+      ECC_RedClosR g (eSig x A B) (eSig x A' B')
+  | R_CongPair (g: ECCenv) (e1 e1' e2 e2' A A': ECCexp) :
+      ECC_RedClosR g e1 e1' ->
+      ECC_RedClosR g e2 e2' ->
+      ECC_RedClosR g A A'   ->
+      ECC_RedClosR g (ePair e1 e2 A) (ePair e1' e2' A')
+  | R_CongApp (g: ECCenv) (e1 e1' e2 e2': ECCexp) :
+      ECC_RedClosR g e1 e1' ->
+      ECC_RedClosR g e2 e2' ->
+      ECC_RedClosR g (eApp e1 e2) (eApp e1' e2')
+  | R_CongFst (g: ECCenv) (V V': ECCexp) :
+      ECC_RedClosR g V V' ->
+      ECC_RedClosR g (eFst V) (eFst V')
+  | R_CongSnd (g: ECCenv) (V V': ECCexp) :
+      ECC_RedClosR g V V' ->
+      ECC_RedClosR g (eSnd V) (eSnd V')
+  | R_CongIf (g: ECCenv) (e e' e1 e1' e2 e2': ECCexp) :
+      ECC_RedClosR g e e' ->
+      ECC_RedClosR g e1 e1' ->
+      ECC_RedClosR g e2 e2' ->
+      ECC_RedClosR g (eIf e e1 e2) (eIf e' e1' e2')
+.
+
+Hint Constructors ECC_RedClosR.
+
+
+
+Inductive ECC_Equiv: ECCenv -> ECCexp -> ECCexp -> Prop :=
+  | E_Equiv (g: ECCenv) (e e1 e2: ECCexp) :
+      ECC_RedClosR g e1 e ->
+      ECC_RedClosR g e2 e ->
+      ECC_Equiv g e1 e2
+  | E_EquivIta1 (g: ECCenv) (e1 A e e2 e2': ECCexp) (x: atom) :
+      ECC_RedClosR g e1 (eAbs x A e) ->
+      ECC_RedClosR g e2 e2' ->
+      ECC_Equiv (gAssum g x A) e (eApp e2' (eId x)) ->
+      ECC_Equiv g e1 e2
+  | E_EquivIta2 (g: ECCenv) (e e1 e1' e2 A : ECCexp) (x: atom) :
+      ECC_RedClosR g e1 e1' ->
+      ECC_RedClosR g e2 (eAbs x A e) ->
+      ECC_Equiv (gAssum g x A) (eApp e1' (eId x)) e ->
+      ECC_Equiv g e1 e2
+  | E_EquivAlpha (g: ECCenv) (e1 e2: ECCexp):
+      ECC_Aeq e1 e2 ->
+      ECC_Equiv g e1 e2
+.
+
+Hint Constructors ECC_Equiv.
+
+(* Typing *)
+
+Inductive ECC_sub_type: ECCenv -> ECCexp -> ECCexp -> Prop :=
+| ST_Cong (g: ECCenv) (A B: ECCexp) :
+  ECC_Equiv g A B ->
+  ECC_sub_type g A B
+| ST_Cum (g: ECCenv) (i: nat) :
+  ECC_sub_type g (eUni (uType i)) (eUni (uType (S i)))
+| ST_Pi (g: ECCenv) (A1 A2 B1 B2: ECCexp) (x1 x2: atom) :
+  (ECC_Equiv g A1 A2) ->
+  (ECC_sub_type (gAssum g x1 A2) B1 (subst x2 (eId x1) B2)) -> (* eId x1 ?*)
+  (ECC_sub_type g (ePi x1 A1 B1) (ePi x2 A2 B2))
+.
+
+Hint Constructors ECC_sub_type.
+
+Inductive ECC_has_type: ECCenv -> ECCexp -> ECCexp -> Prop :=
+| T_Ax_Prop (g: ECCenv) :
+  (ECC_has_type g (eUni uProp) (eUni (uType 0)))
+| T_Ax_Type (g: ECCenv) (i: nat) :
+  (ECC_has_type g (eUni (uType i)) (eUni (uType (S i))))
+| T_Var (g: ECCenv) (x: atom) (A: ECCexp) :
+  (ECC_LookupTypeR g x A) -> (* this needs adjustment *)
+  (ECC_has_type g (eId x) A)
+| T_Let (g: ECCenv) (e e' A B: ECCexp) (x: atom):
+  (ECC_has_type g e A) ->
+  (ECC_has_type (gDef (gAssum g x A) x e) e' B) ->
+  (ECC_has_type g (eLet x e e') (subst x e B))
+| T_Prod_Prop (g: ECCenv) (x: atom) (A B: ECCexp) (i: nat):
+  (ECC_has_type g A (eUni (uType i))) ->
+  (ECC_has_type (gAssum g x A) B (eUni (uProp))) ->
+  (ECC_has_type g (ePi x A B) (eUni (uProp)))
+| T_Prod_Type (g: ECCenv) (x: atom) (A B: ECCexp) (i: nat):
+  (ECC_has_type g A (eUni (uType i))) ->
+  (ECC_has_type (gAssum g x A) B (eUni (uType i))) ->
+  (ECC_has_type g (ePi x A B) (eUni (uType i)))
+| T_Lam (g: ECCenv) (x: atom) (A e B: ECCexp) :
+  (ECC_has_type (gAssum g x A) e B) ->
+  (ECC_has_type g (eAbs x A e) (ePi x A B))
+| T_App (g: ECCenv) (x: atom) (e e' A' B: ECCexp) :
+  (ECC_has_type g e (ePi x A' B)) ->
+  (ECC_has_type g e' A') ->
+  (ECC_has_type g (eApp e e') (subst x e B))
+| T_Sig (g: ECCenv) (x: atom) (A B: ECCexp) (i: nat) :
+  (ECC_has_type g A (eUni (uType i))) ->
+  (ECC_has_type (gAssum g x A) B (eUni (uType i))) -> (* should these be the same i*)
+  (ECC_has_type g (eSig x A B) (eUni (uType i)))
+| T_Pair (g: ECCenv) (e1 e2 A B: ECCexp) (x: atom) :
+  (ECC_has_type g e1 A) ->
+  (ECC_has_type g e2 (subst x e1 B)) ->
+  (ECC_has_type g (ePair e1 e2 (eSig x A B)) (eSig x A B))
+| T_Fst (g: ECCenv) (e A B: ECCexp) (x: atom) :
+  (ECC_has_type g e (eSig x A B)) ->
+  (ECC_has_type g (eFst e) A)
+| T_Snd (g: ECCenv) (e A B: ECCexp) (x: atom) :
+  (ECC_has_type g e (eSig x A B)) ->
+  (ECC_has_type g (eSnd e) (subst x (eFst e) B))
+| T_Bool (g: ECCenv):
+  (ECC_has_type g (eBool) (eUni (uType 0)))
+| T_True (g: ECCenv):
+  (ECC_has_type g (eTru) (eBool))
+| T_False (g: ECCenv):
+  (ECC_has_type g (eFls) (eBool))
+| T_If (g: ECCenv) (B U e e1 e2: ECCexp) (x: atom):
+  (ECC_has_type (gAssum g x (eBool)) B U) ->
+  (ECC_has_type g e (eBool)) ->
+  (ECC_has_type g e1 (subst x (eTru) B)) ->
+  (ECC_has_type g e2 (subst x (eFls) B)) ->
+  (ECC_has_type g (eIf e e1 e2) (subst x e B))
+| T_Conv (g: ECCenv) (e A B U: ECCexp) :
+  (ECC_has_type g e A) ->
+  (ECC_has_type g B U) ->
+  (ECC_sub_type g A B) ->
+  (ECC_has_type g e B)
+.
+
+
+Hint Constructors ECC_has_type.
+
+Goal ECC_has_type gEmpty (eUni uProp) (eUni (uType 0)).
+Proof.
+intuition.
+Qed.
+
+(* ECC Notation *)
+
+Bind Scope ECC_scope with ECCexp.
+Bind Scope ECC_scope with ECCuni.
+Bind Scope ECC_scope with ECCenv.
+Delimit Scope ECC_scope with ECC.
+Coercion eId: atom >-> ECCexp.
+
+Notation "'type' x" := (eUni (uType x)) (at level 50):  ECC_scope.
+Notation "'prop'" := (eUni uProp) (at level 50):  ECC_scope.
+Definition example_Type := (type 3)%ECC: ECCexp.
+Definition example_Prop := (prop)%ECC: ECCexp.
+
+Notation "{ e1 e2 }" := (eApp e1 e2) (at level 50,e1 at level 9):  ECC_scope.
+Definition example_App := { X Y }%ECC: ECCexp.
+
+Notation "'LET' x ':=' A 'in' B" := (eLet x A B) (at level 50, format "'[v' 'LET'  x  ':='  A '/' 'in' '['  B ']' ']'") : ECC_scope.
+Definition example_Let := (LET X := Y in Z)%ECC : ECCexp.
+Print example_Let.
+Definition F:= fresh (X::Y::Z::nil).
+Definition example_Let2 := (LET X := (type 3) in LET F := (LET X := (type 2) in X) in ({X F}))%ECC.
+Print example_Let2.
+
+Notation "'Pi' x : A '->' B" := (ePi x A B) (at level 50, x at level 9, A at level 9) : ECC_scope.
+Definition example_Pi := (Pi X : F -> Y)%ECC : ECCexp.
+Notation "'\'  x : A  '->'  B" := (eAbs x A B) (at level 50, x at level 9, A at level 9) : ECC_scope.
+Definition example_Abs := (\ X: Y -> Z)%ECC : ECCexp.
+Notation "'Sig' x : A '..' B" := (eSig x A B) (at level 50, x at level 1, A at level 1): ECC_scope.
+Definition example_Sig := (Sig X : Y .. Z)%ECC : ECCexp.
+Notation "< e1 , e2 > 'as' A" := (ePair e1 e2 A) (at level 50, e1 at level 5, e2 at level 5, A at level 5): ECC_scope.
+Definition example_Pair := (< X, Y > as (Sig X : Y .. Z))%ECC : ECCexp.
+Notation "'fst' e" := (eFst e) (at level 50, e at level 5): ECC_scope.
+Notation "'snd' e" := (eSnd e) (at level 50, e at level 5): ECC_scope.
+
+Definition example_ycombinator := (\F:(type 3) -> ({(\X:(type 2) -> ({F {X X}})) (\X:(type 2) -> ({F {X X}}))}))%ECC.
+Print example_ycombinator.
+
+Compute subst X Y (LET Y := type 1 in X).
+
+Goal ECC_RedClosR gEmpty (LET X := Y in LET Y := type 1 in X) Y.
+Proof.
+cut (ECC_RedR gEmpty (LET X := Y in LET Y := type 1 in X)%ECC (subst X (eId Y) (LET Y := type 1 in X))%ECC).
+- cut (ECC_RedR gEmpty (subst X (eId Y) (LET Y := type 1 in X))%ECC Y). 
+  + eauto.
+  + cbv. apply R_Let.
+- cbv. apply R_Let.
+Qed.
+
+Goal ECC_has_type gEmpty (fst (<eTru , eFls> as (Sig X : eBool .. eBool))) eBool.
+eauto.
+Qed.
+
+Goal ECC_has_type gEmpty (fst (<eTru , eFls> as 
+                            (Sig X : eBool .. (eIf X eBool (Pi Y : eBool -> eBool))))) eBool.
+Proof.
+eapply T_Fst. eapply T_Pair.
+  - apply T_True.
+  - cbv. apply T_Conv with (A := eBool) (U := (type 0)%ECC).
+    + apply T_False.
+    + eapply T_Conv.
+      * apply T_If with (U:=(type 1)%ECC). 
+        -- auto.
+        -- auto.
+        -- auto.
+        -- cbn. eapply T_Prod_Type.
+          ++ auto.
+          ++ auto.
+      * auto.
+      * cbn. apply ST_Cong. apply E_EquivAlpha. apply aeq_id.
+    + apply ST_Cong. apply E_Equiv with (e:= eBool).
+      * auto.
+      * eauto.
+Unshelve. exact 1.
+Qed.
+   
+
+(* End ECC.*)
+
+(* (* Module ECCA. *)
+ *)
+(* -=ECCA Definition=- *)
+
+(* Restricted ECCA, used in computing *)
+
+Inductive ECCAval: Type :=
+  | avId (x: atom)
+  | avUni (U: ECCuni)
+  | avPi (x: atom) (A B: ECCAconf)
+  | avAbs (x: atom) (A B: ECCAconf)
+  | avSig (x: atom) (A B: ECCAconf)
+  | avPair (v1 v2: ECCAval) (A: ECCAconf)
+  | avTru
+  | avFls
+  | avBool
+with
+ECCAconf: Type :=
+  | acfComp (e: ECCAcomp)
+  | acfLet (x: atom) (A: ECCAcomp) (B: ECCAconf)
+  | acfIf (v: ECCAval) (m1 m2: ECCAconf)
+with
+ECCAcomp: Type :=
+  | acpApp (v1 v2: ECCAval)
+  | acpVal (v: ECCAval)
+  | acpFst (v: ECCAval)
+  | acpSnd (v: ECCAval)
+  | acpSubst (x arg body: ECCAval)
+.
+
+Inductive ECCAcont: Type :=
+  | actHole
+  | actLetHole (x: atom) (B: ECCAconf)
+.
+
+Inductive ECCAenv: Type :=
+  | agEmpty
+  | agAssum (g: ECCAenv) (x: atom) (A: ECCAconf)
+  | agDef (g: ECCAenv) (x: atom) (v: ECCAcomp)
+  | agEq (g: ECCAenv) (v1 v2: ECCAval)
+.
+Inductive ECCAexp: Type :=
+  | eavId (x: atom)
+  | eavUni (U: ECCuni)
+  | eavPi (x: atom) (A B: ECCAexp)
+  | eavAbs (x: atom) (A B: ECCAexp)
+  | eavSig (x: atom) (A B: ECCAexp)
+  | eavPair (v1 v2: ECCAexp) (A: ECCAexp)
+  | eavTru
+  | eavFls
+  | eavBool
+  | eacfComp (e: ECCAexp)
+  | eacfLet (x: atom) (A: ECCAexp) (B: ECCAexp)
+  | eacfIf (v: ECCAexp) (m1 m2: ECCAexp)
+  | eacpApp (v1 v2: ECCAexp)
+  | eacpVal (v: ECCAexp)
+  | eacpFst (v: ECCAexp)
+  | eacpSnd (v: ECCAexp)
+  | eacpSubst (x arg body: ECCAexp)
+.
+
+Fixpoint flattenECCAval (e: ECCAval): ECCAexp :=
+match e with
+  | avId x => eavId x
+  | avUni U => eavUni U
+  | avPi x A B => eavPi x (flattenECCAconf A) (flattenECCAconf B) 
+  | avAbs x A B => eavAbs x (flattenECCAconf A) (flattenECCAconf B)
+  | avSig x A B => eavSig x (flattenECCAconf A) (flattenECCAconf B)
+  | avPair v1 v2 A => eavPair (flattenECCAval v1) (flattenECCAval v2) (flattenECCAconf A)
+  | avTru => eavTru
+  | avFls => eavFls
+  | avBool => eavBool
+end
+with flattenECCAcomp (e: ECCAcomp): ECCAexp :=
+match e with
+  | acpApp v1 v2 => eacpApp (flattenECCAval v1) (flattenECCAval v2)
+  | acpVal v => eacpVal (flattenECCAval v)
+  | acpFst v => eacpFst (flattenECCAval v)
+  | acpSnd v => eacpSnd (flattenECCAval v)
+  | acpSubst x arg body => eacpSubst (flattenECCAval x) (flattenECCAval arg) (flattenECCAval body)
+end
+with flattenECCAconf (e: ECCAconf): ECCAexp :=
+match e with
+  | acfComp e => eacfComp (flattenECCAcomp e)
+  | acfLet x A B => eacfLet x (flattenECCAcomp A) (flattenECCAconf B)
+  | acfIf v m1 m2 => eacfIf (flattenECCAval v) (flattenECCAconf m1) (flattenECCAconf m2)
+end.
+
+
+Coercion acpVal: ECCAval >-> ECCAcomp.
+Coercion acfComp: ECCAcomp >-> ECCAconf.
+
+Inductive ECCA_LookupTypeR : ECCAenv -> atom -> ECCAconf -> Prop:=
+  | aLT_gFirst (g': ECCAenv) (x: atom) (A: ECCAval):
+      ECCA_LookupTypeR (agAssum g' x A) x A
+  | aLT_AssumRest (g: ECCAenv) (x x': atom) (A a': ECCAval):
+      ECCA_LookupTypeR g x A ->
+      (x <> x') ->
+      (ECCA_LookupTypeR (agAssum g x' a') x A)
+  | aLT_DefRest (g: ECCAenv) (x x': atom) (A a': ECCAval):
+      ECCA_LookupTypeR g x A ->
+  (*     (x <> x') -> *)
+      (ECCA_LookupTypeR (agDef g x' a') x A)
+  | aLT_EqRest (g: ECCAenv) (x: atom) (v A v': ECCAval):
+      ECCA_LookupTypeR g x A ->
+      ECCA_LookupTypeR (agEq g v v') x A 
+.
+
+Inductive ECCA_LookupDefR : ECCAenv -> atom -> ECCAcomp -> Prop:=
+  | aLD_gFirst (g': ECCAenv) (x: atom) (e: ECCAcomp) (A: ECCAconf):
+      ECCA_LookupDefR (agAssum (agDef g' x e) x A) x e
+  | aLD_AssumRest (g: ECCAenv) (x x': atom) (e: ECCAcomp) (a': ECCAconf):
+      ECCA_LookupDefR g x e ->
+      (x <> x') ->
+      (ECCA_LookupDefR (agAssum g x' a') x e)
+  | aLD_DefRest (g: ECCAenv) (x x': atom) (e e': ECCAcomp):
+      ECCA_LookupDefR g x e ->
+      (x <> x') ->
+      (ECCA_LookupDefR (agDef g x' e') x e)
+  | aLD_EqRest (g: ECCAenv) (x: atom) (v v': ECCAval) (e: ECCAcomp):
+      ECCA_LookupDefR g x e ->
+      ECCA_LookupDefR (agEq g v v') x e 
+.
+
+(*should change val to conf *)
+Inductive ECCA_LookupEqR : ECCAenv -> ECCAval -> ECCAval -> Prop:=
+  | aLE_gFirst (g': ECCAenv) (v v': ECCAval):
+    ECCA_LookupEqR (agEq g' v v') v v'
+  | aLE_AssumRest (g: ECCAenv) (x : atom) (v v' a: ECCAval):
+      ECCA_LookupEqR g v v' ->
+      (ECCA_LookupEqR (agAssum g x a) v v')
+  | aLE_DefRest (g: ECCAenv) (x: atom) (v v' e: ECCAval):
+      ECCA_LookupEqR g v v' ->
+      (ECCA_LookupEqR (agDef g x e) v v')
+  | aLE_EqRest (g: ECCAenv) (x: atom) (v1 v2 v1' v2': ECCAval):
+      ECCA_LookupEqR g v1 v2 ->
+      (v1 <> v1') ->
+      ECCA_LookupEqR (agEq g v1' v2') v1 v2 
+.
+
+Definition aSubst (x: atom) (arg body: ECCAconf): ECCAconf. Proof. Admitted.
+Definition ECCA_RedClosR: ECCAenv -> ECCAconf -> ECCAconf -> Prop. Proof. Admitted.
+Definition ECCA_Aeq: ECCAconf -> ECCAconf -> Prop. Proof. Admitted.
+
+Definition conf_to_val (e: ECCAconf): option ECCAval :=
+match e with
+  | acfComp c => match c with 
+      | acpVal v => Some v
+      | _ => None
+      end
+  | _ => None
+  end.
+
+Compute (conf_to_val avTru).
+Compute (conf_to_val (acfLet X avTru avTru)).
+Compute (conf_to_val (acpVal avTru)).
+Compute (conf_to_val (acfComp avTru)).
+
+(* Lemma conf_is_val_dec: forall e: ECCAconf, 
+(exists v, (conf_to_val e) = Some v) + (conf_to_val e = None). Proof.
+intros. destruct e; auto.
+  - destruct e; auto.
+    +  *)
+
+Inductive ECCA_Equiv: ECCAenv -> ECCAconf -> ECCAconf -> Prop :=
+  | aE_Equiv (g: ECCAenv) (e e1 e2: ECCAconf) :
+      ECCA_RedClosR g e1 e ->
+      ECCA_RedClosR g e2 e ->
+      ECCA_Equiv g e1 e2
+   | aE_EquivIta1 (g: ECCAenv) (e1 A e e2 e2': ECCAconf) (v2': ECCAval) (x: atom) :
+      ECCA_RedClosR g e1 (avAbs x A e) ->
+      ECCA_RedClosR g e2 e2' ->
+      conf_to_val e2' = Some v2' ->
+      ECCA_Equiv (agAssum g x A) e (acpApp v2' (avId x)) ->
+      ECCA_Equiv g e1 e2 
+   | aE_EquivIta2 (g: ECCAenv) (e e1 e1' e2 A : ECCAconf) (v1': ECCAval) (x: atom) :
+      ECCA_RedClosR g e1 e1' ->
+      ECCA_RedClosR g e2 (avAbs x A e) ->
+      conf_to_val e1' = Some v1' ->
+      ECCA_Equiv (agAssum g x A) (acpApp v1' (avId x)) e ->
+      ECCA_Equiv g e1 e2 
+  | aE_EquivAlpha (g: ECCAenv) (e1 e2: ECCAconf):
+      ECCA_Aeq e1 e2 ->
+      ECCA_Equiv g e1 e2
+  | aE_Subst1 (g: ECCAenv) (e1 e2 v: ECCAval) (e e': ECCAconf):
+      conf_to_val e = Some v ->
+      ECCA_Equiv g e e' ->
+      ECCA_Equiv g (acpSubst e1 e2 v) e'
+  | aE_Subst2 (g: ECCAenv) (e1 e2 v: ECCAval) (e e': ECCAconf):
+      conf_to_val e = Some v ->
+      ECCA_Equiv g e e' ->
+      ECCA_Equiv g e' (acpSubst e1 e2 v)
+.
+
+Inductive ECCA_sub_type: ECCAenv -> ECCAconf -> ECCAconf -> Prop :=
+| aST_Cong (g: ECCAenv) (A B: ECCAconf) :
+  ECCA_Equiv g A B ->
+  ECCA_sub_type g A B
+| aST_Cum (g: ECCAenv) (i: nat) :
+  ECCA_sub_type g (avUni (uType i)) (avUni (uType (S i)))
+| aST_Pi (g: ECCAenv) (A1 A2 B1 B2: ECCAconf) (x1 x2: atom) :
+  (ECCA_Equiv g A1 A2) ->
+  (ECCA_sub_type (agAssum g x1 A2) B1 (aSubst x2 (avId x1) B2)) -> (* eId x1 ?*)
+  (ECCA_sub_type g (avPi x1 A1 B1) (avPi x2 A2 B2))
+.
+
+Inductive ECCA_val_has_type: ECCAenv -> ECCAval -> ECCAconf -> Prop :=
+| aT_Ax_Prop (g: ECCAenv) :
+  (ECCA_val_has_type g (avUni uProp) (avUni (uType 0)))
+| aT_Ax_Type (g: ECCAenv) (i: nat) :
+  (ECCA_val_has_type g (avUni (uType i)) (avUni (uType (S i))))
+| aT_Var (g: ECCAenv) (x: atom) (A: ECCAval) :
+  (ECCA_LookupTypeR g x A) -> (* this needs adjustment *)
+  (ECCA_val_has_type g (avId x) A)
+| aT_Bool (g: ECCAenv):
+  (ECCA_val_has_type g (avBool) (avUni (uType 0)))
+| aT_True (g: ECCAenv):
+  (ECCA_val_has_type g (avTru) (avBool))
+| aT_False (g: ECCAenv):
+  (ECCA_val_has_type g (avFls) (avBool))
+| aT_Sig (g: ECCAenv) (x: atom) (A B: ECCAconf) (i: nat) :
+  (ECCA_conf_has_type g A (avUni (uType i))) ->
+  (ECCA_conf_has_type (agAssum g x A) B (avUni (uType i))) ->
+  (ECCA_val_has_type g (avSig x A B) (avUni (uType i)))
+| aT_Pair (g: ECCAenv) (v1 v2: ECCAval) (A B: ECCAconf) (x: atom) :
+  (ECCA_val_has_type g v1 A) ->
+  (ECCA_val_has_type g v2 (aSubst x v1 B)) ->
+  (ECCA_val_has_type g (avPair v1 v2 (avSig x A B)) (avSig x A B))
+| aT_Prod_Prop (g: ECCAenv) (x: atom) (A B: ECCAconf) (i: nat):
+  (ECCA_conf_has_type g A (avUni (uType i))) ->
+  (ECCA_conf_has_type (agAssum g x A) B (avUni (uProp))) ->
+  (ECCA_val_has_type g (avPi x A B) (avUni (uProp)))
+| aT_Prod_Type (g: ECCAenv) (x: atom) (A B: ECCAconf) (i: nat):
+  (ECCA_conf_has_type g A (avUni (uType i))) ->
+  (ECCA_conf_has_type (agAssum g x A) B (avUni (uType i))) ->
+  (ECCA_val_has_type g (avPi x A B) (avUni (uType i)))
+| aT_Lam (g: ECCAenv) (x: atom) (A e B: ECCAconf) :
+  (ECCA_conf_has_type (agAssum g x A) e B) ->
+  (ECCA_val_has_type g (avAbs x A e) (avPi x A B))
+| aT_ValIsConf (g: ECCAenv) (v: ECCAval) (e: ECCAconf):
+  ECCA_conf_has_type g v e ->
+  ECCA_val_has_type g v e
+with 
+ECCA_conf_has_type: ECCAenv -> ECCAconf -> ECCAconf -> Prop :=
+| aT_Let (g: ECCAenv) (n: ECCAcomp) (m A B: ECCAconf) (x: atom):
+  (ECCA_comp_has_type g n A) ->
+(*should this be (def(assum(g))) or (assum(def(g)))*)
+  (ECCA_conf_has_type (agDef (agAssum g x A) x n) m B) ->
+  (ECCA_conf_has_type g (acfLet x n m) (aSubst x n B))
+| aT_If (g: ECCAenv) (B U e1 e2: ECCAconf) (e: ECCAval) (x: atom):
+  ECCA_conf_has_type (agAssum g x avBool) B U -> 
+  ECCA_val_has_type g e avBool ->
+  ECCA_conf_has_type (agEq g e avTru) e1 (aSubst x avTru B) ->
+  ECCA_conf_has_type (agEq g e avFls) e2 (aSubst x avFls B) -> 
+  ECCA_conf_has_type g (acfIf e e1 e2) (aSubst x e B)
+| aT_Comp (g: ECCAenv) (e: ECCAcomp) (A: ECCAconf):
+  ECCA_comp_has_type g e A ->
+  ECCA_conf_has_type g (acfComp e) A
+| aT_Conv (g: ECCAenv) (e A B U: ECCAconf) :
+  (ECCA_conf_has_type g e A) ->
+  (ECCA_conf_has_type g B U) ->
+  (ECCA_sub_type g A B) ->
+  (ECCA_conf_has_type g e B)
+with
+ECCA_comp_has_type: ECCAenv -> ECCAcomp -> ECCAconf -> Prop :=
+| aT_App (g: ECCAenv) (x: atom) (e e': ECCAval) (A' B: ECCAconf) :
+  (ECCA_val_has_type g e (avPi x A' B)) ->
+  (ECCA_val_has_type g e' A') ->
+  (ECCA_comp_has_type g (acpApp e e') (aSubst x e B))
+| aT_Fst (g: ECCAenv) (e: ECCAval) (A B: ECCAconf) (x: atom) :
+  (ECCA_val_has_type g e (avSig x A B)) ->
+  (ECCA_comp_has_type g (acpFst e) A)
+| aT_Snd (g: ECCAenv) (e: ECCAval) (A B: ECCAconf) (x: atom) :
+  (ECCA_val_has_type g e (avSig x A B)) ->
+  (ECCA_comp_has_type g (acpSnd e) (aSubst x (acpFst e) B)) 
+| aT_Subst (x: atom) (g: ECCAenv) (A B U: ECCAconf) (e e1 e2: ECCAval):
+  (ECCA_conf_has_type (agAssum g x A) B U) ->
+  ECCA_val_has_type g e1 A -> 
+  ECCA_val_has_type g e2 A ->
+  ECCA_val_has_type g e (aSubst x e1 B) ->
+  ECCA_LookupEqR g e1 e2 ->
+  ECCA_comp_has_type g (acpSubst e1 e2 e) (aSubst x e2 B) 
+| aT_Val (g: ECCAenv) (v: ECCAval) (A: ECCAconf):
+  ECCA_val_has_type g v A ->
+  ECCA_comp_has_type g (acpVal v) A
+| aT_CompIsConf (g: ECCAenv) (c: ECCAcomp) (e: ECCAconf):
+  ECCA_conf_has_type g c e ->
+  ECCA_comp_has_type g c e
+.
+
+
+(* -=ECCA Notation=- *)
+
+Bind Scope ECCA_scope with ECCAval.
+Bind Scope ECCA_scope with ECCAconf.
+Bind Scope ECCA_scope with ECCAcomp.
+Bind Scope ECCA_scope with ECCAcont.
+Delimit Scope ECCA_scope with ECCA.
+Coercion avId: atom >-> ECCAval.
+Definition natToAtom (i: nat) : atom := i.
+Coercion natToAtom: nat >-> atom.
+
+Notation "'type' x" := (avUni (uType x)) (at level 50):  ECCA_scope.
+Notation "'prop'" := (avUni uProp) (at level 50):  ECCA_scope.
+Definition example_aType := (type 3)%ECCA: ECCAval.
+Definition example_aProp := (prop)%ECCA: ECCAval.
+
+Notation "{ e1 e2 }" := (acpApp e1 e2) (at level 50,e1 at level 9):  ECCA_scope.
+Definition example_aApp := { X Y }%ECCA: ECCAcomp.
+
+Notation "'LET' x ':=' A 'in' B" := (acfLet x A B) (at level 50, format "'[v' 'LET'  x  ':='  A '/' 'in' '['  B ']' ']'") : ECCA_scope.
+Definition example_aLet := (LET X := Y in Z)%ECCA : ECCAconf.
+Print example_aLet.
+Definition example_aLet2 := (LET X := (type 3) in LET F := (LET X := (type 2) in X) in ({X F}))%ECC.
+Print example_aLet2.
+
+Notation "'P' x : A '->' B" := (avPi x A B) (at level 50, x at level 9, A at level 9) : ECCA_scope.
+Definition example_aPi := (P X : Y -> Z)%ECCA : ECCAval.
+Notation "'\' x : A '->' B" := (avAbs x A B) (at level 50, x at level 9, A at level 9) : ECCA_scope.
+Definition example_aAbs := (\ X : Y -> Z)%ECCA : ECCAval.
+
+Notation "'[]'" := (actHole) (at level 50) : ECCA_scope.
+Definition aHole := []%ECCA.
+Notation "'LET' x ':=' '[]' 'in' B" := (actLetHole x B) (at level 50) : ECCA_scope.
+Definition example_aLetHole := (LET X := [] in X)%ECCA.
+Print example_aLetHole.
+
+Goal ECCA_comp_has_type agEmpty (acpFst (avPair avTru avFls 
+    (avSig X avBool 
+          (acfIf X avBool (avPi Y avBool avBool))))) avBool.
+Proof.
+eapply aT_Fst. eapply aT_Pair.
+  - apply aT_True.
+  - cbv. apply aT_ValIsConf. apply aT_Conv with (A := avBool) (U := (type 0)%ECCA).
+    + apply aT_Comp. apply aT_Val. apply aT_False.
+    + eapply T_Conv.
+      * apply T_If with (U:=(type 1)%ECC). 
+        -- auto.
+        -- auto.
+        -- auto.
+        -- cbn. eapply T_Prod_Type.
+          ++ auto.
+          ++ auto.
+      * auto.
+      * cbn. apply ST_Cong. apply E_EquivAlpha. apply aeq_id.
+    + apply ST_Cong. apply E_Equiv with (e:= eBool).
+      * auto.
+      * eauto.
+Unshelve. exact 1.
+Qed.
+
+
+
+(* End ECCA. *)
+(* 
+Inductive ECCA_Aeq : ECCexp -> ECCexp -> Prop :=
+  | aeq_id (e: ECCexp):
+    ECC_Aeq e e
+  | aeq_var (x: atom):
+     ECC_Aeq (eId x) (eId x)
+  | aeq_abs_same (x: atom) (t1 t2 b1 b2: ECCexp):
+     ECC_Aeq t1 t2 -> 
+     ECC_Aeq b1 b2 ->
+     ECC_Aeq (eAbs x t1 b1) (eAbs x t2 b2)
+  | aeq_abs_diff (x y: atom) (t1 t2 b1 b2: ECCexp):
+     x <> y ->
+     (mem x (FV b2)) = false ->
+     ECC_Aeq b1 (swap y x b2) ->
+     ECC_Aeq t1 t2 ->
+     ECC_Aeq (eAbs x t1 b1) (eAbs y t2 b2)
+  | aeq_pi_same (x: atom) (t1 t2 b1 b2: ECCexp):
+     ECC_Aeq t1 t2 -> 
+     ECC_Aeq b1 b2 ->
+     ECC_Aeq (ePi x t1 b1) (ePi x t2 b2)
+  | aeq_pi_diff (x y: atom) (t1 t2 b1 b2: ECCexp):
+     x <> y ->
+     (mem x (FV b2)) = false ->
+     ECC_Aeq b1 (swap y x b2) ->
+     ECC_Aeq t1 t2 ->
+     ECC_Aeq (ePi x t1 b1) (ePi y t2 b2)
+  | aeq_let_same (x: atom) (t1 t2 b1 b2: ECCexp):
+     ECC_Aeq t1 t2 -> 
+     ECC_Aeq b1 b2 ->
+     ECC_Aeq (eLet x t1 b1) (eLet x t2 b2)
+  | aeq_let_diff (x y: atom) (t1 t2 b1 b2: ECCexp):
+     x <> y ->
+     (mem x (FV b2)) = false ->
+     ECC_Aeq b1 (swap y x b2) ->
+     ECC_Aeq t1 t2 ->
+     ECC_Aeq (eLet x t1 b1) (eLet y t2 b2)
+  | aeq_sig_same (x: atom) (t1 t2 b1 b2: ECCexp):
+     ECC_Aeq t1 t2 -> 
+     ECC_Aeq b1 b2 ->
+     ECC_Aeq (eSig x t1 b1) (eSig x t2 b2)
+  | aeq_sig_diff (x y: atom) (t1 t2 b1 b2: ECCexp):
+     x <> y ->
+     (mem x (FV b2)) = false ->
+     ECC_Aeq b1 (swap y x b2) ->
+     ECC_Aeq t1 t2 ->
+     ECC_Aeq (eSig x t1 b1) (eSig y t2 b2)
+  | aeq_app (t1 t2 t1' t2': ECCexp):
+     ECC_Aeq t1 t1' -> ECC_Aeq t2 t2' ->
+     ECC_Aeq (eApp t1 t2) (eApp t1' t2')
+  | aeq_pair (t1 t2 t1' t2' A A': ECCexp):
+     ECC_Aeq t1 t1' -> ECC_Aeq t2 t2' ->
+     ECC_Aeq A A' ->
+     ECC_Aeq (ePair t1 t2 A) (ePair t1' t2' A')
+  | aeq_eFst (e e': ECCexp):
+     ECC_Aeq e e' ->
+     ECC_Aeq (eFst e) (eFst e')
+  | aeq_eSnd (e e': ECCexp):
+     ECC_Aeq e e' ->
+     ECC_Aeq (eSnd e) (eSnd e')
+  | aeq_if (e1 e2 e3 e1' e2' e3': ECCexp):
+     ECC_Aeq e1 e1' ->
+     ECC_Aeq e2 e2' ->
+     ECC_Aeq e3 e3' ->
+     ECC_Aeq (eIf e1 e2 e3) (eIf e1' e2' e3').
+
+ *)
+(* ===ECC to ECCA translation== *)
+
+
+Fixpoint fill_hole (e: ECCAcomp) (K: ECCAcont): ECCAconf :=
+  match K with
+    | actHole => acfComp e
+    | actLetHole x B => acfLet x e B
+end.
+
+(* Plan: starter function starts namestate at max of atoms in the ECCexp, so all new atoms are higher than old atoms. *)
+
+(* {ns : NameState} *)
+
+Fixpoint trans  (ns: atom) (e: ECCexp) (K: ECCAcont) : ECCAconf :=
+  let X := (S ns) in
+  let Y := (S (S ns)) in
+  let Z := (S (S (S ns))) in
+  match e with
+    | eId x => (fill_hole (acpVal (avId x)) K)
+    | ePi x A B => (fill_hole (acpVal (avPi (x) (trans ns A actHole) (trans ns B actHole))) K)
+    | eAbs x A e => (fill_hole (acpVal (avAbs x (trans ns A actHole) (trans ns e actHole))) K)
+    | eApp e1 e2 =>
+        (trans X e1 (actLetHole X
+            (trans Y e2 (actLetHole Y
+                (fill_hole (acpApp (avId X) (avId Y)) K)))))
+    | eLet x e1 e2 => (trans ns e1 (actLetHole x
+                          (trans (ns) e2 K)))
+    | eSig x A B => (fill_hole (acpVal (avSig x (trans ns A actHole) (trans ns B actHole))) K)
+    | ePair e1 e2 A => (trans X e1 (actLetHole X
+            (trans Y e2 (actLetHole Y
+               (trans Z A (actLetHole Z
+                (fill_hole (avPair (avId X) (avId Y) (avId Z)) K)))))))
+    | eFst e => (trans X e (actLetHole X
+                   (fill_hole (acpFst (avId X)) K)))
+    | eSnd e => (trans X e (actLetHole X
+                   (fill_hole (acpSnd X) K)))
+    | eTru => (fill_hole (acpVal avTru) K)
+    | eFls => (fill_hole (acpVal avFls) K)
+    | eBool=> (fill_hole (acpVal avBool) K)
+    | eUni u => (fill_hole (acpVal (avUni u)) K)
+    | eIf e e1 e2 => (trans X e (actLetHole X 
+                        (acfIf (avId X) 
+                            (trans Y e1 (actLetHole Y (fill_hole (acpSubst X avTru (avId Y)) K)))
+                            (trans Y e1 (actLetHole Y (fill_hole (acpSubst X avFls (avId Y)) K))))))
+end.
+
+Definition transStarter (e: ECCexp):=
+  trans (fresh (FV e)) e actHole
+.
+
+Compute transStarter (LET X := Y in LET Y := type 1 in X)%ECC.
+Compute transStarter (fst (<eTru , eFls> as 
+                            (Sig X : eBool .. (eIf X eBool (Pi Y : eBool -> eBool))))).
